05Closure/Closure.thy
@@ -2,174 +2,228 @@ theory Closure
   imports "../03Debruijn/DebruijnIndices" "../00Utils/Iteration"
 begin
 
-datatype closure = 
-  CConst nat
-  | CLam ty "closure list" expr\<^sub>d
+section \<open>Closures\<close>
 
-datatype cframe = 
-  CApp1 "closure list" expr\<^sub>d
-  | CApp2 closure
-  | CReturn "closure list"
+text \<open>Stack evaluation got rid of one source of recursive tree-walking in our evaluation relation, 
+but another remains: substitution itself. In this stage, we eliminate substitution, replacing it 
+with lookups into explicit environments. This would be simple, except for lambda-abstractions, which
+can be passed around as values, yet contain variables that might have been substituted in for 
+somewhere else long ago. Fortunately this is a long-solved problem. The solution is the closure, a 
+block of code with a private environment it carries around with it, and which can represent a 
+function value: the substituted variables are exactly those in the closure's environment. For us, 
+not having defined any code yet, closures will be expressions with attached environments, but the 
+idea remains the same.\<close>
 
-datatype closure_state = 
-  CSE "cframe list" "closure list"  expr\<^sub>d
-  | CSC "cframe list" closure
+text \<open>We call all these distinguished-datatype values "closure-values", even the ones (like 
+\<open>Const\<^sub>c\<close>) that manifestly do not need to carry an environment; this is just to give them a name. 
+Closure environments, incidentally, are just lists of closure-values, indexed by the variables they 
+replace.\<close>
 
-fun latest_environment :: "cframe list \<rightharpoonup> closure list" where
-  "latest_environment [] = None"
-| "latest_environment (CApp1 cs e # s) = latest_environment s"
-| "latest_environment (CApp2 c # s) = latest_environment s"
-| "latest_environment (CReturn cs # s) = Some cs"
+datatype closure\<^sub>c = 
+  Const\<^sub>c nat
+  | Lam\<^sub>c ty "closure\<^sub>c list" expr\<^sub>d
 
-inductive typecheck_closure :: "closure \<Rightarrow> ty \<Rightarrow> bool" (infix ":\<^sub>c\<^sub>l" 50)
-      and typecheck_closure_list :: "closure list \<Rightarrow> ty list \<Rightarrow> bool" (infix ":\<^sub>c\<^sub>l\<^sub>s" 50) where
-  tcc_const [simp]: "CConst k :\<^sub>c\<^sub>l Num"
-| tcc_lam [simp]: "cs :\<^sub>c\<^sub>l\<^sub>s ts \<Longrightarrow> insert_at 0 t\<^sub>1 ts \<turnstile>\<^sub>d e : t\<^sub>2 \<Longrightarrow> CLam t\<^sub>1 cs e :\<^sub>c\<^sub>l Arrow t\<^sub>1 t\<^sub>2"
-| tcc_nil [simp]: "[] :\<^sub>c\<^sub>l\<^sub>s []"
-| tcc_cons [simp]: "c :\<^sub>c\<^sub>l t \<Longrightarrow> cs :\<^sub>c\<^sub>l\<^sub>s ts \<Longrightarrow> c # cs :\<^sub>c\<^sub>l\<^sub>s t # ts"
+text \<open>Typing closure-values and environments are for the most part easy. The one key thing to note 
+is that in a closure proper, \<open>Lam\<^sub>c t \<Delta> e\<close>, e is almost but not quite a closed expression; it 
+represents a function body and so has a single variable not in \<Delta>, to be replaced by its eventual 
+argument.\<close>
 
-inductive_cases [elim]:"CConst k :\<^sub>c\<^sub>l t"
-inductive_cases [elim]: "CLam t\<^sub>1 cs e :\<^sub>c\<^sub>l t"
-inductive_cases [elim]: "[] :\<^sub>c\<^sub>l\<^sub>s ts"
-inductive_cases [elim]: "c # cs :\<^sub>c\<^sub>l\<^sub>s ts"
+inductive typing_closure\<^sub>c :: "closure\<^sub>c \<Rightarrow> ty \<Rightarrow> bool" (infix ":\<^sub>c\<^sub>l" 50)
+      and typing_environment\<^sub>c :: "closure\<^sub>c list \<Rightarrow> ty list \<Rightarrow> bool" (infix ":\<^sub>c\<^sub>l\<^sub>s" 50) where
+  tc\<^sub>c_const [simp]: "Const\<^sub>c n :\<^sub>c\<^sub>l Num"
+| tc\<^sub>c_lam [simp]: "\<Delta> :\<^sub>c\<^sub>l\<^sub>s \<Gamma> \<Longrightarrow> insert_at 0 t\<^sub>1 \<Gamma> \<turnstile>\<^sub>d e : t\<^sub>2 \<Longrightarrow> Lam\<^sub>c t\<^sub>1 \<Delta> e :\<^sub>c\<^sub>l Arrow t\<^sub>1 t\<^sub>2"
+| tc\<^sub>c_nil [simp]: "[] :\<^sub>c\<^sub>l\<^sub>s []"
+| tc\<^sub>c_cons [simp]: "c :\<^sub>c\<^sub>l t \<Longrightarrow> \<Delta> :\<^sub>c\<^sub>l\<^sub>s \<Gamma> \<Longrightarrow> c # \<Delta> :\<^sub>c\<^sub>l\<^sub>s t # \<Gamma>"
 
-inductive typecheck_cstack :: "cframe list \<Rightarrow> ty \<Rightarrow> ty \<Rightarrow> bool" (infix ":\<^sub>c _ \<rightarrow>" 50) where
-  tcc_snil [simp]: "[] :\<^sub>c t \<rightarrow> t"
-| tcc_scons_app1 [simp]: "cs :\<^sub>c\<^sub>l\<^sub>s ts \<Longrightarrow> ts \<turnstile>\<^sub>d e : t\<^sub>1 \<Longrightarrow> s :\<^sub>c t\<^sub>2 \<rightarrow> t \<Longrightarrow> 
-    latest_environment s = Some cs \<Longrightarrow> CApp1 cs e # s :\<^sub>c Arrow t\<^sub>1 t\<^sub>2 \<rightarrow> t"
-| tcc_scons_app2 [simp]: "c :\<^sub>c\<^sub>l Arrow t\<^sub>1 t\<^sub>2 \<Longrightarrow> s :\<^sub>c t\<^sub>2 \<rightarrow> t \<Longrightarrow> latest_environment s = Some cs \<Longrightarrow> 
-    CApp2 c # s :\<^sub>c t\<^sub>1 \<rightarrow> t"
-| tcc_scons_ret [simp]: "cs :\<^sub>c\<^sub>l\<^sub>s ts \<Longrightarrow> s :\<^sub>c t' \<rightarrow> t \<Longrightarrow> CReturn cs # s :\<^sub>c t' \<rightarrow> t"
-
-inductive_cases [elim]: "[] :\<^sub>c t' \<rightarrow> t"
-inductive_cases [elim]: "CApp1 cs e # s :\<^sub>c t' \<rightarrow> t"
-inductive_cases [elim]: "CApp2 c # s :\<^sub>c t' \<rightarrow> t"
-inductive_cases [elim]: "CReturn cs # s :\<^sub>c t' \<rightarrow> t"
-
-inductive typecheck_closure_state :: "closure_state \<Rightarrow> ty \<Rightarrow> bool" (infix ":\<^sub>c" 50) where
-  tcc_state_ev [simp]: "s :\<^sub>c t' \<rightarrow> t \<Longrightarrow> cs :\<^sub>c\<^sub>l\<^sub>s ts \<Longrightarrow> latest_environment s = Some cs \<Longrightarrow> 
-    ts \<turnstile>\<^sub>d e : t' \<Longrightarrow> CSE s cs e :\<^sub>c t"
-| tcc_state_ret [simp]: "s :\<^sub>c t' \<rightarrow> t \<Longrightarrow> c :\<^sub>c\<^sub>l t' \<Longrightarrow> CSC s c :\<^sub>c t"
-
-inductive_cases [elim]: "CSE s cs e :\<^sub>c t"
-inductive_cases [elim]: "CSC s c :\<^sub>c t"
-
-inductive evalc :: "closure_state \<Rightarrow> closure_state \<Rightarrow> bool" (infix "\<leadsto>\<^sub>c" 50) where
-  evc_var [simp]: "lookup cs x = Some c \<Longrightarrow> CSE s cs (Var\<^sub>d x) \<leadsto>\<^sub>c CSC s c"
-| evc_con [simp]: "CSE s cs (Const\<^sub>d k) \<leadsto>\<^sub>c CSC s (CConst k)"
-| evc_lam [simp]: "CSE s cs (Lam\<^sub>d t e) \<leadsto>\<^sub>c CSC s (CLam t cs e)"
-| evc_app [simp]: "CSE s cs (App\<^sub>d e\<^sub>1 e\<^sub>2) \<leadsto>\<^sub>c CSE (CApp1 cs e\<^sub>2 # s) cs e\<^sub>1"
-| retc_app1 [simp]: "CSC (CApp1 cs e\<^sub>2 # s) c\<^sub>1 \<leadsto>\<^sub>c CSE (CApp2 c\<^sub>1 # s) cs e\<^sub>2"
-| retc_app2 [simp]: "CSC (CApp2 (CLam t cs e\<^sub>1) # s) c\<^sub>2 \<leadsto>\<^sub>c CSE (CReturn (c\<^sub>2 # cs) # s) (c\<^sub>2 # cs) e\<^sub>1"
-| retc_ret [simp]: "CSC (CReturn cs # s) c \<leadsto>\<^sub>c CSC s c"
-
-lemma canonical_basec [dest]: "c :\<^sub>c\<^sub>l Num \<Longrightarrow> \<exists>k. c = CConst k"
-  by (induction c Num rule: typecheck_closure_typecheck_closure_list.inducts(1)) simp_all
-
-lemma canonical_arrowc [dest]: "c :\<^sub>c\<^sub>l Arrow t\<^sub>1 t\<^sub>2 \<Longrightarrow> 
-    \<exists>cs ts e. c = CLam t\<^sub>1 cs e \<and> (cs :\<^sub>c\<^sub>l\<^sub>s ts) \<and> (insert_at 0 t\<^sub>1 ts \<turnstile>\<^sub>d e : t\<^sub>2)"
-  by (induction c "Arrow t\<^sub>1 t\<^sub>2" rule: typecheck_closure_typecheck_closure_list.inducts(1)) auto
+inductive_cases [elim]:"Const\<^sub>c n :\<^sub>c\<^sub>l t"
+inductive_cases [elim]: "Lam\<^sub>c t\<^sub>1 \<Delta> e :\<^sub>c\<^sub>l t"
+inductive_cases [elim]: "[] :\<^sub>c\<^sub>l\<^sub>s \<Gamma>"
+inductive_cases [elim]: "c # \<Delta> :\<^sub>c\<^sub>l\<^sub>s \<Gamma>"
 
 lemma  "c :\<^sub>c\<^sub>l t \<Longrightarrow> True"
-  and [simp]: "cs :\<^sub>c\<^sub>l\<^sub>s \<Gamma> \<Longrightarrow> lookup \<Gamma> x = Some t \<Longrightarrow> \<exists>c. lookup cs x = Some c \<and> c :\<^sub>c\<^sub>l t"
-proof (induction c t and cs \<Gamma> arbitrary: and x 
-       rule: typecheck_closure_typecheck_closure_list.inducts)
-  case (tcc_cons c t cs ts)
-  thus ?case by (induction x) simp_all
+  and lookup_in_env\<^sub>c [simp]: "\<Delta> :\<^sub>c\<^sub>l\<^sub>s \<Gamma> \<Longrightarrow> lookup \<Gamma> x = Some t \<Longrightarrow> \<exists>c. lookup \<Delta> x = Some c \<and> c :\<^sub>c\<^sub>l t"
+proof (induction c t and \<Delta> \<Gamma> arbitrary: and x rule: typing_closure\<^sub>c_typing_environment\<^sub>c.inducts)
+  case (tc\<^sub>c_cons c t \<Delta> \<Gamma>)
+  thus ?case by (cases x) simp_all
 qed simp_all
 
-lemma [simp]: "ts \<turnstile>\<^sub>d e : t \<Longrightarrow> cs :\<^sub>c\<^sub>l\<^sub>s ts \<Longrightarrow> \<exists>\<Sigma>'. CSE s cs e \<leadsto>\<^sub>c \<Sigma>'"
-proof (induction ts e t rule: typing\<^sub>d.induct)
+lemma canonical_num\<^sub>c [dest]: "c :\<^sub>c\<^sub>l Num \<Longrightarrow> \<exists>n. c = Const\<^sub>c n"
+  by (induction c Num rule: typing_closure\<^sub>c_typing_environment\<^sub>c.inducts(1)) simp_all
+
+lemma canonical_arrow\<^sub>c [dest]: "c :\<^sub>c\<^sub>l Arrow t\<^sub>1 t\<^sub>2 \<Longrightarrow> 
+    \<exists>\<Delta> \<Gamma> e. c = Lam\<^sub>c t\<^sub>1 \<Delta> e \<and> (\<Delta> :\<^sub>c\<^sub>l\<^sub>s \<Gamma>) \<and> (insert_at 0 t\<^sub>1 \<Gamma> \<turnstile>\<^sub>d e : t\<^sub>2)"
+  by (induction c "Arrow t\<^sub>1 t\<^sub>2" rule: typing_closure\<^sub>c_typing_environment\<^sub>c.inducts(1)) auto
+
+text \<open>Our stack frames, meanwhile, have become much more complicated. Because the environment of an 
+expression is no longer just implicitly there by substitution, we need to record the current 
+environment for the unevaluated expression in \<open>FApp1\<^sub>c\<close>. Because the expression in \<open>FApp2\<^sub>c\<close> is always 
+evaluated, we replace it with a closure-value. Finally, in \<open>FReturn\<^sub>c\<close>, we record the environment 
+again - this will be necessary in the next stage. We also provide a utility to get the nearest 
+enclosing environment: that is, the one recorded by the last \<open>FReturn\<^sub>c\<close> pushed on the stack.\<close>
+
+datatype frame\<^sub>c = 
+  FApp1\<^sub>c "closure\<^sub>c list" expr\<^sub>d
+  | FApp2\<^sub>c closure\<^sub>c
+  | FReturn\<^sub>c "closure\<^sub>c list"
+
+fun latest_environment :: "frame\<^sub>c list \<rightharpoonup> closure\<^sub>c list" where
+  "latest_environment [] = None"
+| "latest_environment (FApp1\<^sub>c \<Delta> e # s) = latest_environment s"
+| "latest_environment (FApp2\<^sub>c c # s) = latest_environment s"
+| "latest_environment (FReturn\<^sub>c \<Delta> # s) = Some \<Delta>"
+
+text \<open>Typing a stack is about the same as it was last time, given the changes to the frames. But 
+there are a couple of points that might seem unnecessary: we check that the latest environment 
+matches the stored one in \<open>FApp1\<^sub>c\<close> frames; we have nothing to compare it against in \<open>FApp2\<^sub>c\<close>, but 
+check that it at least exists there; and we check that the environment types to something in 
+\<open>FReturn\<^sub>c\<close>. None of these are necessary for the safety proofs here, or the correctness proofs when 
+converting from the stack stage (we could, with sufficient effort, prove them as theorems), but the 
+extra structure guaranteed by these checks will be useful in the next stage.\<close>
+
+inductive typing_stack\<^sub>c :: "frame\<^sub>c list \<Rightarrow> ty \<Rightarrow> ty \<Rightarrow> bool" (infix ":\<^sub>c _ \<rightarrow>" 50) where
+  tcc_snil [simp]: "[] :\<^sub>c t \<rightarrow> t"
+| tcc_scons_app1 [simp]: "\<Delta> :\<^sub>c\<^sub>l\<^sub>s \<Gamma> \<Longrightarrow> \<Gamma> \<turnstile>\<^sub>d e : t\<^sub>1 \<Longrightarrow> s :\<^sub>c t\<^sub>2 \<rightarrow> t \<Longrightarrow> 
+    latest_environment s = Some \<Delta> \<Longrightarrow> FApp1\<^sub>c \<Delta> e # s :\<^sub>c Arrow t\<^sub>1 t\<^sub>2 \<rightarrow> t"
+| tcc_scons_app2 [simp]: "c :\<^sub>c\<^sub>l Arrow t\<^sub>1 t\<^sub>2 \<Longrightarrow> s :\<^sub>c t\<^sub>2 \<rightarrow> t \<Longrightarrow> latest_environment s \<noteq> None \<Longrightarrow> 
+    FApp2\<^sub>c c # s :\<^sub>c t\<^sub>1 \<rightarrow> t"
+| tcc_scons_ret [simp]: "\<Delta> :\<^sub>c\<^sub>l\<^sub>s \<Gamma> \<Longrightarrow> s :\<^sub>c t' \<rightarrow> t \<Longrightarrow> FReturn\<^sub>c \<Delta> # s :\<^sub>c t' \<rightarrow> t"
+
+inductive_cases [elim]: "[] :\<^sub>c t' \<rightarrow> t"
+inductive_cases [elim]: "FApp1\<^sub>c \<Delta> e # s :\<^sub>c t' \<rightarrow> t"
+inductive_cases [elim]: "FApp2\<^sub>c c # s :\<^sub>c t' \<rightarrow> t"
+inductive_cases [elim]: "FReturn\<^sub>c \<Delta> # s :\<^sub>c t' \<rightarrow> t"
+
+text \<open>The evaluation state has also been complicated a little. Because expressions and 
+closure-values are now two distinct datatypes, the evaluated flag has been replaced by two distinct 
+data constructors, one with an expression and environment to be evaluated, the other with a 
+closure-value to be returned. Both, of course, retain the call stack.\<close>
+
+datatype state\<^sub>c = 
+  SE\<^sub>c "frame\<^sub>c list" "closure\<^sub>c list" expr\<^sub>d
+  | SC\<^sub>c "frame\<^sub>c list" closure\<^sub>c
+
+primrec final\<^sub>c :: "state\<^sub>c \<Rightarrow> bool" where
+  "final\<^sub>c (SE\<^sub>c s \<Delta> e) = False"
+| "final\<^sub>c (SC\<^sub>c s c) = (s = [])"
+
+text \<open>Typechecking the state remains much the same, with again a seemingly-redundant environment
+consistency check that will be useful to us later.\<close>
+
+inductive typecheck_state\<^sub>c :: "state\<^sub>c \<Rightarrow> ty \<Rightarrow> bool" (infix ":\<^sub>c" 50) where
+  tcc_state_ev [simp]: "s :\<^sub>c t' \<rightarrow> t \<Longrightarrow> \<Delta> :\<^sub>c\<^sub>l\<^sub>s \<Gamma> \<Longrightarrow> latest_environment s = Some \<Delta> \<Longrightarrow> 
+    \<Gamma> \<turnstile>\<^sub>d e : t' \<Longrightarrow> SE\<^sub>c s \<Delta> e :\<^sub>c t"
+| tcc_state_ret [simp]: "s :\<^sub>c t' \<rightarrow> t \<Longrightarrow> c :\<^sub>c\<^sub>l t' \<Longrightarrow> SC\<^sub>c s c :\<^sub>c t"
+
+inductive_cases [elim]: "SE\<^sub>c s \<Delta> e :\<^sub>c t"
+inductive_cases [elim]: "SC\<^sub>c s c :\<^sub>c t"
+
+text \<open>Evaluation now makes use of the environments, shuffling them between the state environment 
+slot and the stack frames, and looking up variables in them as appropriate. (Although the state as a 
+whole has no free variables, for the first time the expression under examination might.)\<close>
+
+inductive eval\<^sub>c :: "state\<^sub>c \<Rightarrow> state\<^sub>c \<Rightarrow> bool" (infix "\<leadsto>\<^sub>c" 50) where
+  ev\<^sub>c_var [simp]: "lookup \<Delta> x = Some c \<Longrightarrow> SE\<^sub>c s \<Delta> (Var\<^sub>d x) \<leadsto>\<^sub>c SC\<^sub>c s c"
+| ev\<^sub>c_con [simp]: "SE\<^sub>c s \<Delta> (Const\<^sub>d n) \<leadsto>\<^sub>c SC\<^sub>c s (Const\<^sub>c n)"
+| ev\<^sub>c_lam [simp]: "SE\<^sub>c s \<Delta> (Lam\<^sub>d t e) \<leadsto>\<^sub>c SC\<^sub>c s (Lam\<^sub>c t \<Delta> e)"
+| ev\<^sub>c_app [simp]: "SE\<^sub>c s \<Delta> (App\<^sub>d e\<^sub>1 e\<^sub>2) \<leadsto>\<^sub>c SE\<^sub>c (FApp1\<^sub>c \<Delta> e\<^sub>2 # s) \<Delta> e\<^sub>1"
+| ret\<^sub>c_app1 [simp]: "SC\<^sub>c (FApp1\<^sub>c \<Delta> e\<^sub>2 # s) c\<^sub>1 \<leadsto>\<^sub>c SE\<^sub>c (FApp2\<^sub>c c\<^sub>1 # s) \<Delta> e\<^sub>2"
+| ret\<^sub>c_app2 [simp]: "SC\<^sub>c (FApp2\<^sub>c (Lam\<^sub>c t \<Delta> e\<^sub>1) # s) c\<^sub>2 \<leadsto>\<^sub>c SE\<^sub>c (FReturn\<^sub>c (c\<^sub>2 # \<Delta>) # s) (c\<^sub>2 # \<Delta>) e\<^sub>1"
+| ret\<^sub>c_ret [simp]: "SC\<^sub>c (FReturn\<^sub>c \<Delta> # s) c \<leadsto>\<^sub>c SC\<^sub>c s c"
+
+text \<open>And the safety theorems:\<close>
+
+lemma eval\<^sub>c_from_nonvalue [simp]: "\<Gamma> \<turnstile>\<^sub>d e : t \<Longrightarrow> \<Delta> :\<^sub>c\<^sub>l\<^sub>s \<Gamma> \<Longrightarrow> \<exists>\<Sigma>'. SE\<^sub>c s \<Delta> e \<leadsto>\<^sub>c \<Sigma>'"
+proof (induction \<Gamma> e t rule: typing\<^sub>d.induct)
   case (tc\<^sub>d_var \<Gamma> x t)
-  then obtain c where "lookup cs x = Some c \<and> c :\<^sub>c\<^sub>l t" by fastforce
-  hence "CSE s cs (Var\<^sub>d x) \<leadsto>\<^sub>c CSC s c" by simp
+  then obtain c where "lookup \<Delta> x = Some c \<and> c :\<^sub>c\<^sub>l t" by fastforce
+  hence "SE\<^sub>c s \<Delta> (Var\<^sub>d x) \<leadsto>\<^sub>c SC\<^sub>c s c" by simp
   thus ?case by fastforce 
 next
-  case (tc\<^sub>d_const \<Gamma> k)
-  have "CSE s cs (Const\<^sub>d k) \<leadsto>\<^sub>c CSC s (CConst k)" by simp
+  case (tc\<^sub>d_const \<Gamma> n)
+  have "SE\<^sub>c s \<Delta> (Const\<^sub>d n) \<leadsto>\<^sub>c SC\<^sub>c s (Const\<^sub>c n)" by simp
   thus ?case by fastforce 
 next
   case (tc\<^sub>d_lam t\<^sub>1 \<Gamma> e t\<^sub>2)
-  have "CSE s cs (Lam\<^sub>d t\<^sub>1 e) \<leadsto>\<^sub>c CSC s (CLam t\<^sub>1 cs e)" by simp
+  have "SE\<^sub>c s \<Delta> (Lam\<^sub>d t\<^sub>1 e) \<leadsto>\<^sub>c SC\<^sub>c s (Lam\<^sub>c t\<^sub>1 \<Delta> e)" by simp
   thus ?case by fastforce 
 next
   case (tc\<^sub>d_app \<Gamma> e\<^sub>1 t\<^sub>1 t\<^sub>2 e\<^sub>2)
-  have "CSE s cs (App\<^sub>d e\<^sub>1 e\<^sub>2) \<leadsto>\<^sub>c CSE (CApp1 cs e\<^sub>2 # s) cs e\<^sub>1" by simp
+  have "SE\<^sub>c s \<Delta> (App\<^sub>d e\<^sub>1 e\<^sub>2) \<leadsto>\<^sub>c SE\<^sub>c (FApp1\<^sub>c \<Delta> e\<^sub>2 # s) \<Delta> e\<^sub>1" by simp
   then show ?case by fastforce
 qed
 
-lemma [simp]: "s :\<^sub>c t' \<rightarrow> t \<Longrightarrow> c :\<^sub>c\<^sub>l t' \<Longrightarrow> s = [] \<or> (\<exists>\<Sigma>'. CSC s c \<leadsto>\<^sub>c \<Sigma>')"
-proof (induction s t' t rule: typecheck_cstack.induct)
-  case (tcc_scons_app1 cs ts e\<^sub>2 t\<^sub>1 s t\<^sub>2 t)
-  moreover hence "CSC (CApp1 cs e\<^sub>2 # s) c \<leadsto>\<^sub>c CSE (CApp2 c # s) cs e\<^sub>2" by simp
+lemma eval\<^sub>c_from_value [simp]: "s :\<^sub>c t' \<rightarrow> t \<Longrightarrow> c :\<^sub>c\<^sub>l t' \<Longrightarrow> s = [] \<or> (\<exists>\<Sigma>'. SC\<^sub>c s c \<leadsto>\<^sub>c \<Sigma>')"
+proof (induction s t' t rule: typing_stack\<^sub>c.induct)
+  case (tcc_scons_app1 \<Delta> \<Gamma> e\<^sub>2 t\<^sub>1 s t\<^sub>2 t)
+  moreover hence "SC\<^sub>c (FApp1\<^sub>c \<Delta> e\<^sub>2 # s) c \<leadsto>\<^sub>c SE\<^sub>c (FApp2\<^sub>c c # s) \<Delta> e\<^sub>2" by simp
   ultimately show ?case by fastforce
 next
   case (tcc_scons_app2 c\<^sub>1 t\<^sub>1 t\<^sub>2 s t)
-  then obtain cs ts e where "c\<^sub>1 = CLam t\<^sub>1 cs e \<and> (cs :\<^sub>c\<^sub>l\<^sub>s ts) \<and> (insert_at 0 t\<^sub>1 ts \<turnstile>\<^sub>d e : t\<^sub>2)" 
+  then obtain \<Delta> ts e where "c\<^sub>1 = Lam\<^sub>c t\<^sub>1 \<Delta> e \<and> (\<Delta> :\<^sub>c\<^sub>l\<^sub>s ts) \<and> (insert_at 0 t\<^sub>1 ts \<turnstile>\<^sub>d e : t\<^sub>2)" 
     by blast
-  moreover hence "CSC (CApp2 (CLam t\<^sub>1 cs e) # s) c \<leadsto>\<^sub>c CSE (CReturn (c # cs) # s) (c # cs) e" by simp
+  moreover hence "SC\<^sub>c (FApp2\<^sub>c (Lam\<^sub>c t\<^sub>1 \<Delta> e) # s) c \<leadsto>\<^sub>c SE\<^sub>c (FReturn\<^sub>c (c # \<Delta>) # s) (c # \<Delta>) e" by simp
   ultimately show ?case by fastforce
 next
-  case (tcc_scons_ret cs ts s t' t)
-  have "CSC (CReturn cs # s) c \<leadsto>\<^sub>c CSC s c" by simp
+  case (tcc_scons_ret \<Delta> \<Gamma> s t' t)
+  have "SC\<^sub>c (FReturn\<^sub>c \<Delta> # s) c \<leadsto>\<^sub>c SC\<^sub>c s c" by simp
   thus ?case by fastforce
 qed simp_all
 
-theorem progressc: "\<Sigma> :\<^sub>c t \<Longrightarrow> (\<exists>c. \<Sigma> = CSC [] c) \<or> (\<exists>\<Sigma>'. \<Sigma> \<leadsto>\<^sub>c \<Sigma>')"
-  by (induction \<Sigma> t rule: typecheck_closure_state.induct) simp_all
+theorem progress\<^sub>c: "\<Sigma> :\<^sub>c t \<Longrightarrow> final\<^sub>c \<Sigma> \<or> (\<exists>\<Sigma>'. \<Sigma> \<leadsto>\<^sub>c \<Sigma>')"
+  by (induction \<Sigma> t rule: typecheck_state\<^sub>c.induct) simp_all
 
-theorem preservationc [simp]: "\<Sigma> \<leadsto>\<^sub>c \<Sigma>' \<Longrightarrow> \<Sigma> :\<^sub>c t \<Longrightarrow> \<Sigma>' :\<^sub>c t"
-proof (induction \<Sigma> \<Sigma>' rule: evalc.induct)
-  case (evc_var cs x c s)
-  then obtain t' ts where X: "s :\<^sub>c t' \<rightarrow> t" and "(cs :\<^sub>c\<^sub>l\<^sub>s ts) \<and> lookup ts x = Some t'" by blast
-  then obtain c' where "lookup cs x = Some c' \<and> c' :\<^sub>c\<^sub>l t'" by fastforce
-  with evc_var X show ?case by simp
+theorem preservation\<^sub>c [simp]: "\<Sigma> \<leadsto>\<^sub>c \<Sigma>' \<Longrightarrow> \<Sigma> :\<^sub>c t \<Longrightarrow> \<Sigma>' :\<^sub>c t"
+proof (induction \<Sigma> \<Sigma>' rule: eval\<^sub>c.induct)
+  case (ev\<^sub>c_var \<Delta> x c s)
+  then obtain t' \<Gamma> where X: "s :\<^sub>c t' \<rightarrow> t" and "(\<Delta> :\<^sub>c\<^sub>l\<^sub>s \<Gamma>) \<and> lookup \<Gamma> x = Some t'" by blast
+  then obtain c' where "lookup \<Delta> x = Some c' \<and> c' :\<^sub>c\<^sub>l t'" by fastforce
+  with ev\<^sub>c_var X show ?case by simp
 next
-  case (evc_app s cs e\<^sub>1 e\<^sub>2)
-  then obtain t\<^sub>1 t\<^sub>2 ts where "(s :\<^sub>c t\<^sub>2 \<rightarrow> t) \<and> (ts \<turnstile>\<^sub>d e\<^sub>2 : t\<^sub>1)" 
-   and X: "(cs :\<^sub>c\<^sub>l\<^sub>s ts) \<and> latest_environment s = Some cs \<and> (ts \<turnstile>\<^sub>d e\<^sub>1 : Arrow t\<^sub>1 t\<^sub>2)" by blast
-  hence "CApp1 cs e\<^sub>2 # s :\<^sub>c Arrow t\<^sub>1 t\<^sub>2 \<rightarrow> t"  by fastforce
+  case (ev\<^sub>c_app s \<Delta> e\<^sub>1 e\<^sub>2)
+  then obtain t\<^sub>1 t\<^sub>2 \<Gamma> where "(s :\<^sub>c t\<^sub>2 \<rightarrow> t) \<and> (\<Gamma> \<turnstile>\<^sub>d e\<^sub>2 : t\<^sub>1)" 
+   and X: "(\<Delta> :\<^sub>c\<^sub>l\<^sub>s \<Gamma>) \<and> latest_environment s = Some \<Delta> \<and> (\<Gamma> \<turnstile>\<^sub>d e\<^sub>1 : Arrow t\<^sub>1 t\<^sub>2)" by blast
+  hence "FApp1\<^sub>c \<Delta> e\<^sub>2 # s :\<^sub>c Arrow t\<^sub>1 t\<^sub>2 \<rightarrow> t"  by fastforce
   with X show ?case by fastforce
 next
-  case (retc_app1 cs e\<^sub>2 s c\<^sub>1)
-  then obtain ts t\<^sub>1 t\<^sub>2 where X: "(cs :\<^sub>c\<^sub>l\<^sub>s ts) \<and> latest_environment s = Some cs \<and> (ts \<turnstile>\<^sub>d e\<^sub>2 : t\<^sub>1)" 
+  case (ret\<^sub>c_app1 \<Delta> e\<^sub>2 s c\<^sub>1)
+  then obtain \<Gamma> t\<^sub>1 t\<^sub>2 where X: "(\<Delta> :\<^sub>c\<^sub>l\<^sub>s \<Gamma>) \<and> latest_environment s = Some \<Delta> \<and> (\<Gamma> \<turnstile>\<^sub>d e\<^sub>2 : t\<^sub>1)" 
    and "(s :\<^sub>c t\<^sub>2 \<rightarrow> t) \<and> (c\<^sub>1 :\<^sub>c\<^sub>l Arrow t\<^sub>1 t\<^sub>2)" by blast
-  hence "CApp2 c\<^sub>1 # s :\<^sub>c t\<^sub>1 \<rightarrow> t" by fastforce
+  hence "FApp2\<^sub>c c\<^sub>1 # s :\<^sub>c t\<^sub>1 \<rightarrow> t" by fastforce
   with X show ?case by fastforce
 next
-  case (retc_app2 t\<^sub>1 cs e\<^sub>1 s c\<^sub>2)
-  then obtain ts t\<^sub>2 where X: "s :\<^sub>c t\<^sub>2 \<rightarrow> t" and Y: "insert_at 0 t\<^sub>1 ts \<turnstile>\<^sub>d e\<^sub>1 : t\<^sub>2" 
-   and "(cs :\<^sub>c\<^sub>l\<^sub>s ts) \<and> (c\<^sub>2 :\<^sub>c\<^sub>l t\<^sub>1)" by blast
-  hence Z: "c\<^sub>2 # cs :\<^sub>c\<^sub>l\<^sub>s insert_at 0 t\<^sub>1 ts" by (induction ts) simp_all
-  with X have "CReturn (c\<^sub>2 # cs) # s :\<^sub>c t\<^sub>2 \<rightarrow> t" by simp
+  case (ret\<^sub>c_app2 t\<^sub>1 \<Delta> e\<^sub>1 s c\<^sub>2)
+  then obtain \<Gamma> t\<^sub>2 where X: "s :\<^sub>c t\<^sub>2 \<rightarrow> t" and Y: "insert_at 0 t\<^sub>1 \<Gamma> \<turnstile>\<^sub>d e\<^sub>1 : t\<^sub>2" 
+   and "(\<Delta> :\<^sub>c\<^sub>l\<^sub>s \<Gamma>) \<and> (c\<^sub>2 :\<^sub>c\<^sub>l t\<^sub>1)" by blast
+  hence Z: "c\<^sub>2 # \<Delta> :\<^sub>c\<^sub>l\<^sub>s insert_at 0 t\<^sub>1 \<Gamma>" by (induction \<Gamma>) simp_all
+  with X have "FReturn\<^sub>c (c\<^sub>2 # \<Delta>) # s :\<^sub>c t\<^sub>2 \<rightarrow> t" by simp
   with Y Z show ?case by fastforce
 qed fastforce+
 
-lemma [simp]: "iter (\<leadsto>\<^sub>c) \<Sigma> \<Sigma>' \<Longrightarrow> \<Sigma> :\<^sub>c t \<Longrightarrow> \<Sigma>' :\<^sub>c t"
+lemma preservation\<^sub>c_iter [simp]: "iter (\<leadsto>\<^sub>c) \<Sigma> \<Sigma>' \<Longrightarrow> \<Sigma> :\<^sub>c t \<Longrightarrow> \<Sigma>' :\<^sub>c t"
   by (induction \<Sigma> \<Sigma>' rule: iter.induct) simp_all
 
-theorem determinismc: "\<Sigma> \<leadsto>\<^sub>c \<Sigma>' \<Longrightarrow> \<Sigma> \<leadsto>\<^sub>c \<Sigma>'' \<Longrightarrow> \<Sigma>' = \<Sigma>''"
-proof (induction \<Sigma> \<Sigma>' rule: evalc.induct)
-  case (evc_var cs x c s)
-  from evc_var(2, 1) show ?case by (induction "CSE s cs (Var\<^sub>d x)" \<Sigma>'' rule: evalc.induct) simp_all 
+theorem determinism\<^sub>c: "\<Sigma> \<leadsto>\<^sub>c \<Sigma>' \<Longrightarrow> \<Sigma> \<leadsto>\<^sub>c \<Sigma>'' \<Longrightarrow> \<Sigma>' = \<Sigma>''"
+proof (induction \<Sigma> \<Sigma>' rule: eval\<^sub>c.induct)
+  case (ev\<^sub>c_var \<Delta> x c s)
+  from ev\<^sub>c_var(2, 1) show ?case by (induction rule: eval\<^sub>c.cases) simp_all 
 next
-  case (evc_con s cs k)
-  thus ?case by (induction "CSE s cs (Const\<^sub>d k)" \<Sigma>'' rule: evalc.induct) simp_all 
+  case (ev\<^sub>c_con s \<Delta> k)
+  thus ?case by (induction rule: eval\<^sub>c.cases) simp_all 
 next
-  case (evc_lam s cs t e)
-  thus ?case by (induction "CSE s cs (Lam\<^sub>d t e)" \<Sigma>'' rule: evalc.induct) simp_all 
+  case (ev\<^sub>c_lam s \<Delta> t e)
+  thus ?case by (induction rule: eval\<^sub>c.cases) simp_all 
 next
-  case (evc_app s cs e\<^sub>1 e\<^sub>2)
-  thus ?case by (induction "CSE s cs (App\<^sub>d e\<^sub>1 e\<^sub>2)" \<Sigma>'' rule: evalc.induct) simp_all 
+  case (ev\<^sub>c_app s \<Delta> e\<^sub>1 e\<^sub>2)
+  thus ?case by (induction rule: eval\<^sub>c.cases) simp_all 
 next
-  case (retc_app1 cs e\<^sub>2 s c\<^sub>1)
-  thus ?case by (induction "CSC (CApp1 cs e\<^sub>2 # s) c\<^sub>1" \<Sigma>'' rule: evalc.induct) simp_all 
+  case (ret\<^sub>c_app1 \<Delta> e\<^sub>2 s c\<^sub>1)
+  thus ?case by (induction rule: eval\<^sub>c.cases) simp_all 
 next
-  case (retc_app2 t cs e\<^sub>1 s c\<^sub>2)
-  thus ?case by (induction "CSC (CApp2 (CLam t cs e\<^sub>1) # s) c\<^sub>2" \<Sigma>'' rule: evalc.induct) simp_all 
+  case (ret\<^sub>c_app2 t \<Delta> e\<^sub>1 s c\<^sub>2)
+  thus ?case by (induction rule: eval\<^sub>c.cases) simp_all 
 next
-  case (retc_ret cs s c)
-  thus ?case by (induction "CSC (CReturn cs # s) c" \<Sigma>'' rule: evalc.induct) simp_all 
+  case (ret\<^sub>c_ret \<Delta> s c)
+  thus ?case by (induction rule: eval\<^sub>c.cases) simp_all 
 qed
 
 end
