05Closure/ClosureConversion.thy
@@ -2,30 +2,30 @@ theory ClosureConversion
   imports Closure "../04Stack/Stack" "../03Debruijn/Multisubst"
 begin
 
-primrec declosure :: "closure \<Rightarrow> expr\<^sub>d" where
-  "declosure (CConst k) = Const\<^sub>d k"
-| "declosure (CLam t cs e) = multisubst (map declosure cs) (Lam\<^sub>d t e)"
+primrec declosure :: "closure\<^sub>c \<Rightarrow> expr\<^sub>d" where
+  "declosure (Const\<^sub>c k) = Const\<^sub>d k"
+| "declosure (Lam\<^sub>c t cs e) = multisubst (map declosure cs) (Lam\<^sub>d t e)"
 
-fun declosure_stack :: "cframe list \<Rightarrow> frame\<^sub>k list" where
+fun declosure_stack :: "frame\<^sub>c list \<Rightarrow> frame\<^sub>k list" where
   "declosure_stack [] = []"
-| "declosure_stack (CApp1 cs e # s) = FApp1\<^sub>k (multisubst (map declosure cs) e) # declosure_stack s"
-| "declosure_stack (CApp2 c # s) = FApp2\<^sub>k (declosure c) # declosure_stack s"
-| "declosure_stack (CReturn cs # s) = FReturn\<^sub>k # declosure_stack s"
+| "declosure_stack (FApp1\<^sub>c cs e # s) = FApp1\<^sub>k (multisubst (map declosure cs) e) # declosure_stack s"
+| "declosure_stack (FApp2\<^sub>c c # s) = FApp2\<^sub>k (declosure c) # declosure_stack s"
+| "declosure_stack (FReturn\<^sub>c cs # s) = FReturn\<^sub>k # declosure_stack s"
 
-primrec declosure_state :: "closure_state \<Rightarrow> state\<^sub>k" where
-  "declosure_state (CSE s cs e) = S\<^sub>k False (declosure_stack s) (multisubst (map declosure cs) e)"
-| "declosure_state (CSC s c) = S\<^sub>k True (declosure_stack s) (declosure c)"
+primrec destate\<^sub>c :: "state\<^sub>c \<Rightarrow> state\<^sub>k" where
+  "destate\<^sub>c (SE\<^sub>c s cs e) = S\<^sub>k False (declosure_stack s) (multisubst (map declosure cs) e)"
+| "destate\<^sub>c (SC\<^sub>c s c) = S\<^sub>k True (declosure_stack s) (declosure c)"
 
 lemma [simp]: "value\<^sub>d (declosure c)"
 proof (induction c)
-  case (CLam t cs e)
+  case (Lam\<^sub>c t cs e)
   thus ?case by (induction cs arbitrary: e) simp_all
 qed simp_all
 
 lemma [simp]: "c :\<^sub>c\<^sub>l t \<Longrightarrow> [] \<turnstile>\<^sub>d declosure c : t"
   and [simp]: "cs :\<^sub>c\<^sub>l\<^sub>s ts \<Longrightarrow> tc_expr_context ts (map declosure cs)" 
-proof (induction c t and cs ts rule: typecheck_closure_typecheck_closure_list.inducts)
-  case (tcc_lam cs ts t\<^sub>1 e t\<^sub>2)
+proof (induction c t and cs ts rule: typing_closure\<^sub>c_typing_environment\<^sub>c.inducts)
+  case (tc\<^sub>c_lam cs ts t\<^sub>1 e t\<^sub>2)
   then obtain e' where "multisubst (map declosure cs) (Lam\<^sub>d t\<^sub>1 e) = Lam\<^sub>d t\<^sub>1 e' \<and> ([t\<^sub>1] \<turnstile>\<^sub>d e' : t\<^sub>2) \<and> 
     (\<forall>e\<^sub>2. ([] \<turnstile>\<^sub>d e\<^sub>2 : t\<^sub>1) \<longrightarrow> multisubst (map declosure cs) (subst\<^sub>d 0 e\<^sub>2 e) = subst\<^sub>d 0 e\<^sub>2 e')" 
       by fastforce
@@ -33,7 +33,7 @@ proof (induction c t and cs ts rule: typecheck_closure_typecheck_closure_list.in
 qed simp_all
 
 lemma [simp]: "s :\<^sub>c t' \<rightarrow> t \<Longrightarrow> declosure_stack s :\<^sub>k t' \<rightarrow> t"
-proof (induction s t' t rule: typecheck_cstack.induct)
+proof (induction s t' t rule: typing_stack\<^sub>c.induct)
   case (tcc_scons_app1 cs ts e t\<^sub>1 s t\<^sub>2 t)
   hence "tc_expr_context ts (map declosure cs)" by simp
   moreover from tcc_scons_app1 have "ts \<turnstile>\<^sub>d e : t\<^sub>1" by simp
@@ -46,8 +46,8 @@ next
   ultimately show ?case by simp
 qed simp_all
   
-theorem typesafec [simp]: "\<Sigma> :\<^sub>c t \<Longrightarrow> declosure_state \<Sigma> :\<^sub>k t"
-proof (induction \<Sigma> t rule: typecheck_closure_state.induct)
+theorem typesafec [simp]: "\<Sigma> :\<^sub>c t \<Longrightarrow> destate\<^sub>c \<Sigma> :\<^sub>k t"
+proof (induction \<Sigma> t rule: typecheck_state\<^sub>c.induct)
   case (tcc_state_ev s t' t cs ts e)
   hence "tc_expr_context ts (map declosure cs)" by simp
   moreover from tcc_state_ev have "ts \<turnstile>\<^sub>d e : t'" by simp
@@ -63,8 +63,8 @@ qed
 
 lemma multisubst_closure [simp]: "c :\<^sub>c\<^sub>l t \<Longrightarrow> multisubst es (declosure c) = declosure c"
   and [simp]: "cs :\<^sub>c\<^sub>l\<^sub>s ts \<Longrightarrow> v \<in> set (map declosure cs) \<Longrightarrow> multisubst es v = v"
-proof (induction c t and cs ts rule: typecheck_closure_typecheck_closure_list.inducts)
-  case (tcc_lam cs ts t\<^sub>1 e t\<^sub>2)
+proof (induction c t and cs ts rule: typing_closure\<^sub>c_typing_environment\<^sub>c.inducts)
+  case (tc\<^sub>c_lam cs ts t\<^sub>1 e t\<^sub>2)
   moreover hence "tc_expr_context ts (map declosure cs)" by simp
   ultimately obtain e' where E: "multisubst (map declosure cs) (Lam\<^sub>d t\<^sub>1 e) = Lam\<^sub>d t\<^sub>1 e' \<and> 
     ([t\<^sub>1] \<turnstile>\<^sub>d e' : t\<^sub>2) \<and> (\<forall>e\<^sub>2. ([] \<turnstile>\<^sub>d e\<^sub>2 : t\<^sub>1) \<longrightarrow> 
@@ -81,16 +81,16 @@ proof -
   thus ?thesis by simp
 qed
 
-theorem correctc: "\<Sigma> \<leadsto>\<^sub>c \<Sigma>' \<Longrightarrow> \<Sigma> :\<^sub>c t \<Longrightarrow> iter (\<leadsto>\<^sub>k) (declosure_state \<Sigma>) (declosure_state \<Sigma>')"
-proof (induction \<Sigma> \<Sigma>' rule: evalc.induct)
-  case (evc_var cs x c s)
+theorem correctc: "\<Sigma> \<leadsto>\<^sub>c \<Sigma>' \<Longrightarrow> \<Sigma> :\<^sub>c t \<Longrightarrow> iter (\<leadsto>\<^sub>k) (destate\<^sub>c \<Sigma>) (destate\<^sub>c \<Sigma>')"
+proof (induction \<Sigma> \<Sigma>' rule: eval\<^sub>c.induct)
+  case (ev\<^sub>c_var cs x c s)
   then obtain t' ts where "(s :\<^sub>c t' \<rightarrow> t) \<and> (cs :\<^sub>c\<^sub>l\<^sub>s ts) \<and> lookup ts x = Some t'" by fastforce
   hence "\<And>v es. v \<in> set (map declosure cs) \<Longrightarrow> multisubst es v = v" by auto
-  moreover from evc_var have "lookup (map declosure cs) x = Some (declosure c)" by simp
+  moreover from ev\<^sub>c_var have "lookup (map declosure cs) x = Some (declosure c)" by simp
   ultimately have "multisubst (map declosure cs) (Var\<^sub>d x) = declosure c" by (metis multisubst_var)
   thus ?case by simp
 next
-  case (evc_lam s cs t e)
+  case (ev\<^sub>c_lam s cs t e)
   obtain e' where "multisubst (map declosure cs) (Lam\<^sub>d t e) = Lam\<^sub>d t e'" by fastforce
   hence "S\<^sub>k False (declosure_stack s) (multisubst (map declosure cs) (Lam\<^sub>d t e)) \<leadsto>\<^sub>k
     S\<^sub>k True (declosure_stack s) (multisubst (map declosure cs) (Lam\<^sub>d t e))" by simp
@@ -99,7 +99,7 @@ next
       by (metis iter_step iter_refl)
   thus ?case by simp
 next
-  case (evc_app s cs e\<^sub>1 e\<^sub>2)
+  case (ev\<^sub>c_app s cs e\<^sub>1 e\<^sub>2)
   have "S\<^sub>k False (declosure_stack s) (App\<^sub>d (multisubst (map declosure cs) e\<^sub>1) 
     (multisubst (map declosure cs) e\<^sub>2)) \<leadsto>\<^sub>k 
       S\<^sub>k False (FApp1\<^sub>k (multisubst (map declosure cs) e\<^sub>2) # declosure_stack s) 
@@ -110,7 +110,7 @@ next
         (multisubst (map declosure cs) e\<^sub>1))" by (metis iter_step iter_refl)
   thus ?case by simp
 next
-  case (retc_app1 cs e\<^sub>2 s c\<^sub>1)
+  case (ret\<^sub>c_app1 cs e\<^sub>2 s c\<^sub>1)
   have "S\<^sub>k True (FApp1\<^sub>k (multisubst (map declosure cs) e\<^sub>2) # declosure_stack s) (declosure c\<^sub>1) \<leadsto>\<^sub>k
     S\<^sub>k False (FApp2\<^sub>k (declosure c\<^sub>1) # declosure_stack s) (multisubst (map declosure cs) e\<^sub>2)" by simp
   hence "iter (\<leadsto>\<^sub>k) (S\<^sub>k True (FApp1\<^sub>k (multisubst (map declosure cs) e\<^sub>2) # declosure_stack s) 
@@ -119,7 +119,7 @@ next
         by (metis iter_step iter_refl)
   thus ?case by simp
 next
-  case (retc_app2 t\<^sub>1 cs e\<^sub>1 s c\<^sub>2)
+  case (ret\<^sub>c_app2 t\<^sub>1 cs e\<^sub>1 s c\<^sub>2)
   then obtain ts t\<^sub>2 where T: "(cs :\<^sub>c\<^sub>l\<^sub>s ts) \<and> (insert_at 0 t\<^sub>1 ts \<turnstile>\<^sub>d e\<^sub>1 : t\<^sub>2) \<and> (s :\<^sub>c t\<^sub>2 \<rightarrow> t) \<and> 
     (c\<^sub>2 :\<^sub>c\<^sub>l t\<^sub>1)" by fastforce
   hence "tc_expr_context ts (map declosure cs) \<and> insert_at 0 t\<^sub>1 ts \<turnstile>\<^sub>d e\<^sub>1 : t\<^sub>2" by simp
@@ -137,7 +137,7 @@ next
     by (metis iter_step iter_refl)
   thus ?case by simp
 next
-  case (retc_ret cs s c)
+  case (ret\<^sub>c_ret cs s c)
   have "S\<^sub>k True (FReturn\<^sub>k # declosure_stack s) (declosure c) \<leadsto>\<^sub>k 
     S\<^sub>k True (declosure_stack s) (declosure c)" by simp
   hence "iter (\<leadsto>\<^sub>k) (S\<^sub>k True (FReturn\<^sub>k # declosure_stack s) (declosure c)) 
@@ -148,21 +148,21 @@ qed simp_all
 lemma [simp]: "[] = declosure_stack s \<Longrightarrow> s = []"
   by (induction s rule: declosure_stack.induct) simp_all
 
-lemma [simp]: "FApp1\<^sub>k e # s = declosure_stack s\<^sub>c \<Longrightarrow> \<exists>cs e' s\<^sub>c'. s\<^sub>c = CApp1 cs e' # s\<^sub>c' \<and> 
+lemma [simp]: "FApp1\<^sub>k e # s = declosure_stack s\<^sub>c \<Longrightarrow> \<exists>cs e' s\<^sub>c'. s\<^sub>c = FApp1\<^sub>c cs e' # s\<^sub>c' \<and> 
     e = multisubst (map declosure cs) e' \<and> s = declosure_stack s\<^sub>c'"
   by (induction s\<^sub>c rule: declosure_stack.induct) simp_all
 
 lemma [simp]: "FApp2\<^sub>k e # s = declosure_stack s\<^sub>c \<Longrightarrow> 
-    \<exists>c s\<^sub>c'. s\<^sub>c = CApp2 c # s\<^sub>c' \<and> e = declosure c \<and> s = declosure_stack s\<^sub>c'"
+    \<exists>c s\<^sub>c'. s\<^sub>c = FApp2\<^sub>c c # s\<^sub>c' \<and> e = declosure c \<and> s = declosure_stack s\<^sub>c'"
   by (induction s\<^sub>c rule: declosure_stack.induct) simp_all
 
-lemma [simp]: "FReturn\<^sub>k # s = declosure_stack s\<^sub>c \<Longrightarrow> \<exists>cs s\<^sub>c'. s\<^sub>c = CReturn cs # s\<^sub>c'"
+lemma [simp]: "FReturn\<^sub>k # s = declosure_stack s\<^sub>c \<Longrightarrow> \<exists>cs s\<^sub>c'. s\<^sub>c = FReturn\<^sub>c cs # s\<^sub>c'"
   by (induction s\<^sub>c rule: declosure_stack.induct) simp_all
 
-lemma [dest]: "S\<^sub>k b s e = declosure_state \<Sigma> \<Longrightarrow> 
+lemma [dest]: "S\<^sub>k b s e = destate\<^sub>c \<Sigma> \<Longrightarrow> 
   \<exists>s'. s = declosure_stack s' \<and> 
-    ((\<exists>cs e'. \<not> b \<and> \<Sigma> = CSE s' cs e' \<and> e = multisubst (map declosure cs) e') \<or> 
-      (\<exists>c. b \<and> \<Sigma> = CSC s' c \<and> e = declosure c))"
+    ((\<exists>cs e'. \<not> b \<and> \<Sigma> = SE\<^sub>c s' cs e' \<and> e = multisubst (map declosure cs) e') \<or> 
+      (\<exists>c. b \<and> \<Sigma> = SC\<^sub>c s' c \<and> e = declosure c))"
   by (induction \<Sigma>) simp_all
 
 lemma [dest]: "App\<^sub>d e\<^sub>1 e\<^sub>2 = multisubst (map declosure cs) (Lam\<^sub>d t e) \<Longrightarrow> False"
@@ -173,11 +173,11 @@ proof -
 qed
 
 lemma lam_to_declosure [simp]: "Lam\<^sub>d t\<^sub>1 e = declosure c \<Longrightarrow> c :\<^sub>c\<^sub>l Arrow t' t\<^sub>2 \<Longrightarrow>
-  \<exists>cs e'. c = CLam t\<^sub>1 cs e' \<and> multisubst (map declosure cs) (Lam\<^sub>d t\<^sub>1 e') = Lam\<^sub>d t\<^sub>1 e \<and> 
+  \<exists>cs e'. c = Lam\<^sub>c t\<^sub>1 cs e' \<and> multisubst (map declosure cs) (Lam\<^sub>d t\<^sub>1 e') = Lam\<^sub>d t\<^sub>1 e \<and> 
     ([t\<^sub>1] \<turnstile>\<^sub>d e : t\<^sub>2) \<and> t' = t\<^sub>1 \<and>
     (\<forall>e\<^sub>2. ([] \<turnstile>\<^sub>d e\<^sub>2 : t\<^sub>1) \<longrightarrow> multisubst (map declosure cs) (subst\<^sub>d 0 e\<^sub>2 e') = subst\<^sub>d 0 e\<^sub>2 e)"
 proof (induction c)
-  case (CLam tt cs e')
+  case (Lam\<^sub>c tt cs e')
   moreover then obtain ts where T: "(cs :\<^sub>c\<^sub>l\<^sub>s ts) \<and> (insert_at 0 t' ts \<turnstile>\<^sub>d e' : t\<^sub>2) \<and> tt = t'" 
     by fastforce
   moreover hence "tc_expr_context ts (map declosure cs)" by simp
@@ -185,7 +185,7 @@ proof (induction c)
     ([t'] \<turnstile>\<^sub>d e'' : t\<^sub>2) \<and>
     (\<forall>e\<^sub>2. ([] \<turnstile>\<^sub>d e\<^sub>2 : t') \<longrightarrow> multisubst (map declosure cs) (subst\<^sub>d 0 e\<^sub>2 e') = subst\<^sub>d 0 e\<^sub>2 e'')"
       by fastforce
-  with CLam T show ?case by simp
+  with Lam\<^sub>c T show ?case by simp
 qed simp_all
 
 lemma [dest]: "App\<^sub>d e\<^sub>1 e\<^sub>2 = declosure c \<Longrightarrow> False"
@@ -193,7 +193,7 @@ lemma [dest]: "App\<^sub>d e\<^sub>1 e\<^sub>2 = declosure c \<Longrightarrow> F
 
 lemma [dest]: "App\<^sub>d e\<^sub>1 e\<^sub>2 = multisubst (map declosure cs) (declosure c) \<Longrightarrow> False"
 proof (induction c)
-  case (CLam t cs' e)
+  case (Lam\<^sub>c t cs' e)
   moreover obtain e' where "multisubst (map declosure cs') (Lam\<^sub>d t e) = Lam\<^sub>d t e'" by fastforce
   ultimately show ?case by auto
 qed simp_all 
@@ -205,19 +205,19 @@ lemma [simp]: "App\<^sub>d e\<^sub>1 e\<^sub>2 = multisubst (map declosure cs) e
     e\<^sub>1 = multisubst (map declosure cs) e\<^sub>1' \<and> e\<^sub>2 = multisubst (map declosure cs) e\<^sub>2'"
   by (induction e) auto
 
-lemma [dest]: "Const\<^sub>d k = multisubst es (declosure c) \<Longrightarrow> c = CConst k"
+lemma [dest]: "Const\<^sub>d k = multisubst es (declosure c) \<Longrightarrow> c = Const\<^sub>c k"
 proof (induction c)
-  case (CLam t cs e)
+  case (Lam\<^sub>c t cs e)
   moreover obtain e' where "multisubst (map declosure cs) (Lam\<^sub>d t e) = Lam\<^sub>d t e'" by fastforce
   moreover obtain e'' where "multisubst es (Lam\<^sub>d t e') = Lam\<^sub>d t e''" by fastforce
   ultimately show ?case by simp
 qed simp_all
 
-lemma [dest]: "Const\<^sub>d k = multisubst (map declosure cs) (Var\<^sub>d x) \<Longrightarrow> lookup cs x = Some (CConst k)"
+lemma [dest]: "Const\<^sub>d k = multisubst (map declosure cs) (Var\<^sub>d x) \<Longrightarrow> lookup cs x = Some (Const\<^sub>c k)"
   by (induction cs x rule: lookup.induct) auto
 
 lemma [dest]: "Const\<^sub>d k = multisubst (map declosure cs) e \<Longrightarrow>
-    e = Const\<^sub>d k \<or> (\<exists>x. e = Var\<^sub>d x \<and> lookup cs x = Some (CConst k))"
+    e = Const\<^sub>d k \<or> (\<exists>x. e = Var\<^sub>d x \<and> lookup cs x = Some (Const\<^sub>c k))"
 proof (induction e)
   case (Lam\<^sub>d t e)
   moreover then obtain e' where "multisubst (map declosure cs) (Lam\<^sub>d t e) = Lam\<^sub>d t e'" by force
@@ -228,58 +228,57 @@ lemma [simp]: "c :\<^sub>c\<^sub>l t \<Longrightarrow> incr\<^sub>d x (declosure
   and [simp]: "cs :\<^sub>c\<^sub>l\<^sub>s ts \<Longrightarrow> ts \<turnstile>\<^sub>d e : tt \<Longrightarrow> 
     incr\<^sub>d x (multisubst (map declosure cs) e) = multisubst (map declosure cs) e"
 proof (induction c t and cs ts arbitrary: and e tt 
-       rule: typecheck_closure_typecheck_closure_list.inducts)
-  case (tcc_lam cs ts t\<^sub>1 e t\<^sub>2)
+       rule: typing_closure\<^sub>c_typing_environment\<^sub>c.inducts)
+  case (tc\<^sub>c_lam cs ts t\<^sub>1 e t\<^sub>2)
   moreover hence "ts \<turnstile>\<^sub>d Lam\<^sub>d t\<^sub>1 e : Arrow t\<^sub>1 t\<^sub>2" by simp
   ultimately have "incr\<^sub>d x (multisubst (map declosure cs) (Lam\<^sub>d t\<^sub>1 e)) = 
     multisubst (map declosure cs) (Lam\<^sub>d t\<^sub>1 e)" by blast
   thus ?case by simp
 next
-  case (tcc_cons c t cs ts)
+  case (tc\<^sub>c_cons c t cs ts)
   hence "[] \<turnstile>\<^sub>d declosure c : t" by simp
   hence "ts \<turnstile>\<^sub>d declosure c : t" using tc_postpend by fastforce
-  moreover from tcc_cons have "insert_at 0 t ts \<turnstile>\<^sub>d e : tt" by (cases ts) simp_all
+  moreover from tc\<^sub>c_cons have "insert_at 0 t ts \<turnstile>\<^sub>d e : tt" by (cases ts) simp_all
   ultimately have "ts \<turnstile>\<^sub>d subst\<^sub>d 0 (declosure c) e : tt" by simp
-  with tcc_cons show ?case by simp
+  with tc\<^sub>c_cons show ?case by simp
 qed simp_all
 
 lemma [simp]: "c :\<^sub>c\<^sub>l t \<Longrightarrow> True"
   and [simp]: "cs :\<^sub>c\<^sub>l\<^sub>s ts \<Longrightarrow> insert_at 0 t\<^sub>1 ts \<turnstile>\<^sub>d e : t\<^sub>2 \<Longrightarrow> 
   multisubst (map declosure cs') (multisubst (map declosure cs) (Lam\<^sub>d t\<^sub>1 e)) = 
     multisubst (map declosure cs) (Lam\<^sub>d t\<^sub>1 e)"
-proof (induction c t and cs ts arbitrary: and e 
-       rule: typecheck_closure_typecheck_closure_list.inducts)
-  case tcc_nil
+proof (induction c t and cs ts arbitrary: and e rule: typing_closure\<^sub>c_typing_environment\<^sub>c.inducts)
+  case tc\<^sub>c_nil
   thus ?case by (induction cs') simp_all
 next
-  case (tcc_cons c t cs ts)
+  case (tc\<^sub>c_cons c t cs ts)
   hence "[] \<turnstile>\<^sub>d declosure c : t" by simp
   hence "insert_at 0 t\<^sub>1 ts \<turnstile>\<^sub>d declosure c : t" using tc_postpend by fastforce
-  with tcc_cons show ?case by (cases ts) simp_all
+  with tc\<^sub>c_cons show ?case by (cases ts) simp_all
 qed simp_all
 
 lemma [dest]: "c :\<^sub>c\<^sub>l tt \<Longrightarrow> Lam\<^sub>d t e = multisubst (map declosure cs) (declosure c) \<Longrightarrow>
-  \<exists>cs' e'. c = CLam t cs' e' \<and> 
+  \<exists>cs' e'. c = Lam\<^sub>c t cs' e' \<and> 
     multisubst (map declosure cs') (Lam\<^sub>d t e') = multisubst (map declosure cd) (declosure c)"
 proof (induction c)
-  case (CLam t\<^sub>1 cs' e')
+  case (Lam\<^sub>c t\<^sub>1 cs' e')
   then obtain t\<^sub>2 ts where T: "tt = Arrow t\<^sub>1 t\<^sub>2 \<and> (cs' :\<^sub>c\<^sub>l\<^sub>s ts) \<and> (insert_at 0 t\<^sub>1 ts \<turnstile>\<^sub>d e' : t\<^sub>2)" 
     by fastforce
   hence M: "multisubst (map declosure cs') (Lam\<^sub>d t\<^sub>1 e') = 
       multisubst (map declosure cd) (multisubst (map declosure cs') (Lam\<^sub>d t\<^sub>1 e'))" by fastforce
   obtain e2 where E: "multisubst (map declosure cs') (Lam\<^sub>d t\<^sub>1 e') = Lam\<^sub>d t\<^sub>1 e2" by fastforce
   obtain e3 where "multisubst (map declosure cs) (Lam\<^sub>d t\<^sub>1 e2) = Lam\<^sub>d t\<^sub>1 e3" by fastforce
-  with CLam M E show ?case by simp
+  with Lam\<^sub>c M E show ?case by simp
 qed simp_all
 
 lemma [dest]: "cs :\<^sub>c\<^sub>l\<^sub>s ts \<Longrightarrow> lookup ts x = Some tt \<Longrightarrow> 
   Lam\<^sub>d t e = multisubst (map declosure cs) (Var\<^sub>d x) \<Longrightarrow> 
-    \<exists>cs' e'. lookup cs x = Some (CLam t cs' e') \<and> 
+    \<exists>cs' e'. lookup cs x = Some (Lam\<^sub>c t cs' e') \<and> 
       multisubst (map declosure cs') (Lam\<^sub>d t e') = multisubst (map declosure cs) (Var\<^sub>d x)"
   by (induction cs x arbitrary: ts rule: lookup.induct) fastforce+
 
 lemma [dest]: "cs :\<^sub>c\<^sub>l\<^sub>s ts \<Longrightarrow> ts \<turnstile>\<^sub>d e : t' \<Longrightarrow> Lam\<^sub>d t e' = multisubst (map declosure cs) e \<Longrightarrow> 
-  (\<exists>e''. e = Lam\<^sub>d t e'') \<or> (\<exists>x cs' e''. e = Var\<^sub>d x \<and> lookup cs x = Some (CLam t cs' e'') \<and> 
+  (\<exists>e''. e = Lam\<^sub>d t e'') \<or> (\<exists>x cs' e''. e = Var\<^sub>d x \<and> lookup cs x = Some (Lam\<^sub>c t cs' e'') \<and> 
     multisubst (map declosure cs') (Lam\<^sub>d t e'') = Lam\<^sub>d t e')"
 proof (induction e)
   case (Lam\<^sub>d t e)
@@ -291,50 +290,50 @@ lemma [simp]: "lookup cs x = Some c \<Longrightarrow> c :\<^sub>c\<^sub>l t \<Lo
     multisubst (map declosure cs) (Var\<^sub>d x) = declosure c"
   by (induction cs x rule: lookup.induct) simp_all
 
-lemma [simp]: "value\<^sub>d (multisubst (map declosure cs) e) \<Longrightarrow> CSE s cs e :\<^sub>c t \<Longrightarrow>
-  \<exists>c. CSE s cs e \<leadsto>\<^sub>c CSC s c \<and> multisubst (map declosure cs) e = declosure c"
+lemma [simp]: "value\<^sub>d (multisubst (map declosure cs) e) \<Longrightarrow> SE\<^sub>c s cs e :\<^sub>c t \<Longrightarrow>
+  \<exists>c. SE\<^sub>c s cs e \<leadsto>\<^sub>c SC\<^sub>c s c \<and> multisubst (map declosure cs) e = declosure c"
 proof (induction e)
   case (Var\<^sub>d x)
   then obtain t' ts where "(s :\<^sub>c t' \<rightarrow> t) \<and> (cs :\<^sub>c\<^sub>l\<^sub>s ts) \<and> (lookup ts x = Some t')" by fastforce
   then obtain c where "lookup cs x = Some c \<and> c :\<^sub>c\<^sub>l t'" by fastforce
-  hence "CSE s cs (Var\<^sub>d x) \<leadsto>\<^sub>c CSC s c \<and> multisubst (map declosure cs) (Var\<^sub>d x) = declosure c" 
+  hence "SE\<^sub>c s cs (Var\<^sub>d x) \<leadsto>\<^sub>c SC\<^sub>c s c \<and> multisubst (map declosure cs) (Var\<^sub>d x) = declosure c" 
     by fastforce
   thus ?case by blast
 next
   case (Const\<^sub>d k)
-  have "CSE s cs (Const\<^sub>d k) \<leadsto>\<^sub>c CSC s (CConst k) \<and> 
-    multisubst (map declosure cs) (Const\<^sub>d k) = declosure (CConst k)" by simp
+  have "SE\<^sub>c s cs (Const\<^sub>d k) \<leadsto>\<^sub>c SC\<^sub>c s (Const\<^sub>c k) \<and> 
+    multisubst (map declosure cs) (Const\<^sub>d k) = declosure (Const\<^sub>c k)" by simp
   thus ?case by blast
 next
   case (Lam\<^sub>d tt e)
-  hence "CSE s cs (Lam\<^sub>d tt e) \<leadsto>\<^sub>c CSC s (CLam tt cs e) \<and> 
-    multisubst (map declosure cs) (Lam\<^sub>d tt e) = declosure (CLam tt cs e)" by simp
+  hence "SE\<^sub>c s cs (Lam\<^sub>d tt e) \<leadsto>\<^sub>c SC\<^sub>c s (Lam\<^sub>c tt cs e) \<and> 
+    multisubst (map declosure cs) (Lam\<^sub>d tt e) = declosure (Lam\<^sub>c tt cs e)" by simp
   thus ?case by blast
 qed simp_all
 
-theorem completec [simp]: "declosure_state \<Sigma>\<^sub>c \<leadsto>\<^sub>k \<Sigma>\<^sub>s' \<Longrightarrow> \<Sigma>\<^sub>c :\<^sub>c t \<Longrightarrow> 
-    \<exists>\<Sigma>\<^sub>c'. iter (\<leadsto>\<^sub>c) \<Sigma>\<^sub>c \<Sigma>\<^sub>c' \<and> \<Sigma>\<^sub>s' = declosure_state \<Sigma>\<^sub>c'"
-proof (induction "declosure_state \<Sigma>\<^sub>c" \<Sigma>\<^sub>s' rule: eval\<^sub>k.induct)
+theorem completec [simp]: "destate\<^sub>c \<Sigma>\<^sub>c \<leadsto>\<^sub>k \<Sigma>\<^sub>s' \<Longrightarrow> \<Sigma>\<^sub>c :\<^sub>c t \<Longrightarrow> 
+    \<exists>\<Sigma>\<^sub>c'. iter (\<leadsto>\<^sub>c) \<Sigma>\<^sub>c \<Sigma>\<^sub>c' \<and> \<Sigma>\<^sub>s' = destate\<^sub>c \<Sigma>\<^sub>c'"
+proof (induction "destate\<^sub>c \<Sigma>\<^sub>c" \<Sigma>\<^sub>s' rule: eval\<^sub>k.induct)
   case (ev\<^sub>k_const s k)
-  then obtain s' cs e' where S: "s = declosure_stack s' \<and> \<Sigma>\<^sub>c = CSE s' cs e' \<and> 
+  then obtain s' cs e' where S: "s = declosure_stack s' \<and> \<Sigma>\<^sub>c = SE\<^sub>c s' cs e' \<and> 
     Const\<^sub>d k = multisubst (map declosure cs) e'" by fastforce
   thus ?case
   proof (cases "e' = Const\<^sub>d k")
     case True
-    have "CSE s' cs (Const\<^sub>d k) \<leadsto>\<^sub>c CSC s' (CConst k)" by simp
-    hence "iter (\<leadsto>\<^sub>c) (CSE s' cs (Const\<^sub>d k)) (CSC s' (CConst k))" by (metis iter_refl iter_step)
+    have "SE\<^sub>c s' cs (Const\<^sub>d k) \<leadsto>\<^sub>c SC\<^sub>c s' (Const\<^sub>c k)" by simp
+    hence "iter (\<leadsto>\<^sub>c) (SE\<^sub>c s' cs (Const\<^sub>d k)) (SC\<^sub>c s' (Const\<^sub>c k))" by (metis iter_refl iter_step)
     with S True show ?thesis by fastforce
   next
     case False
-    with S obtain x where E: "e' = Var\<^sub>d x \<and> lookup cs x = Some (CConst k)" by fastforce
-    hence "CSE s' cs (Var\<^sub>d x) \<leadsto>\<^sub>c CSC s' (CConst k)" by simp
-    hence X: "iter (\<leadsto>\<^sub>c) (CSE s' cs (Var\<^sub>d x)) (CSC s' (CConst k))" by simp
-    from S have "S\<^sub>k True s (Const\<^sub>d k) = declosure_state (CSC s' (CConst k))" by simp
+    with S obtain x where E: "e' = Var\<^sub>d x \<and> lookup cs x = Some (Const\<^sub>c k)" by fastforce
+    hence "SE\<^sub>c s' cs (Var\<^sub>d x) \<leadsto>\<^sub>c SC\<^sub>c s' (Const\<^sub>c k)" by simp
+    hence X: "iter (\<leadsto>\<^sub>c) (SE\<^sub>c s' cs (Var\<^sub>d x)) (SC\<^sub>c s' (Const\<^sub>c k))" by simp
+    from S have "S\<^sub>k True s (Const\<^sub>d k) = destate\<^sub>c (SC\<^sub>c s' (Const\<^sub>c k))" by simp
     with S E X show ?thesis by blast
   qed
 next
   case (ev\<^sub>k_lam s tt e)
-  then obtain s' cs e' where S: "s = declosure_stack s' \<and> \<Sigma>\<^sub>c = CSE s' cs e' \<and> 
+  then obtain s' cs e' where S: "s = declosure_stack s' \<and> \<Sigma>\<^sub>c = SE\<^sub>c s' cs e' \<and> 
     Lam\<^sub>d tt e = multisubst (map declosure cs) e'" by fastforce
   with ev\<^sub>k_lam obtain t' ts where T: "(s' :\<^sub>c t' \<rightarrow> t) \<and> (cs :\<^sub>c\<^sub>l\<^sub>s ts) \<and> 
     latest_environment s' = Some cs \<and> ts \<turnstile>\<^sub>d e' : t'" by fastforce
@@ -342,106 +341,106 @@ next
   proof (cases "\<exists>e''. e' = Lam\<^sub>d tt e''")
     case True
     then obtain e'' where E: "e' = Lam\<^sub>d tt e''" by fastforce
-    have "CSE s' cs (Lam\<^sub>d tt e'') \<leadsto>\<^sub>c CSC s' (CLam tt cs e'')" by simp
-    hence "iter (\<leadsto>\<^sub>c) (CSE s' cs (Lam\<^sub>d tt e'')) (CSC s' (CLam tt cs e''))" 
+    have "SE\<^sub>c s' cs (Lam\<^sub>d tt e'') \<leadsto>\<^sub>c SC\<^sub>c s' (Lam\<^sub>c tt cs e'')" by simp
+    hence "iter (\<leadsto>\<^sub>c) (SE\<^sub>c s' cs (Lam\<^sub>d tt e'')) (SC\<^sub>c s' (Lam\<^sub>c tt cs e''))" 
       by (metis iter_refl iter_step)
     with S E show ?thesis by fastforce
   next
     case False
-    with S T obtain x cs' e'' where E: "e' = Var\<^sub>d x \<and> lookup cs x = Some (CLam tt cs' e'') \<and> 
+    with S T obtain x cs' e'' where E: "e' = Var\<^sub>d x \<and> lookup cs x = Some (Lam\<^sub>c tt cs' e'') \<and> 
       multisubst (map declosure cs') (Lam\<^sub>d tt e'') = Lam\<^sub>d tt e" by blast
-    hence "CSE s' cs (Var\<^sub>d x) \<leadsto>\<^sub>c CSC s' (CLam tt cs' e'')" by simp
-    hence X: "iter (\<leadsto>\<^sub>c) (CSE s' cs (Var\<^sub>d x)) (CSC s' (CLam tt cs' e''))" by simp
+    hence "SE\<^sub>c s' cs (Var\<^sub>d x) \<leadsto>\<^sub>c SC\<^sub>c s' (Lam\<^sub>c tt cs' e'')" by simp
+    hence X: "iter (\<leadsto>\<^sub>c) (SE\<^sub>c s' cs (Var\<^sub>d x)) (SC\<^sub>c s' (Lam\<^sub>c tt cs' e''))" by simp
     from S E have "multisubst (map declosure cs) e' = multisubst (map declosure cs') (Lam\<^sub>d tt e'')"
       by metis
-    with S have "S\<^sub>k True s (Lam\<^sub>d tt e) = declosure_state (CSC s' (CLam tt cs' e''))" by simp
+    with S have "S\<^sub>k True s (Lam\<^sub>d tt e) = destate\<^sub>c (SC\<^sub>c s' (Lam\<^sub>c tt cs' e''))" by simp
     with S E X show ?thesis by blast
   qed
 next
   case (ev\<^sub>k_app1 s e\<^sub>1 e\<^sub>2)
-  then obtain s' cs e' where S: "s = declosure_stack s' \<and> \<Sigma>\<^sub>c = CSE s' cs e' \<and> 
+  then obtain s' cs e' where S: "s = declosure_stack s' \<and> \<Sigma>\<^sub>c = SE\<^sub>c s' cs e' \<and> 
     App\<^sub>d e\<^sub>1 e\<^sub>2 = multisubst (map declosure cs) e'" by fastforce
   then obtain e\<^sub>1' e\<^sub>2' where E: "e' = App\<^sub>d e\<^sub>1' e\<^sub>2' \<and>
     e\<^sub>1 = multisubst (map declosure cs) e\<^sub>1' \<and> e\<^sub>2 = multisubst (map declosure cs) e\<^sub>2'" by fastforce                                                  
-  have "CSE s' cs (App\<^sub>d e\<^sub>1' e\<^sub>2') \<leadsto>\<^sub>c CSE (CApp1 cs e\<^sub>2' # s') cs e\<^sub>1'" by simp
-  hence "iter (\<leadsto>\<^sub>c) (CSE s' cs (App\<^sub>d e\<^sub>1' e\<^sub>2')) (CSE (CApp1 cs e\<^sub>2' # s') cs e\<^sub>1')" 
+  have "SE\<^sub>c s' cs (App\<^sub>d e\<^sub>1' e\<^sub>2') \<leadsto>\<^sub>c SE\<^sub>c (FApp1\<^sub>c cs e\<^sub>2' # s') cs e\<^sub>1'" by simp
+  hence "iter (\<leadsto>\<^sub>c) (SE\<^sub>c s' cs (App\<^sub>d e\<^sub>1' e\<^sub>2')) (SE\<^sub>c (FApp1\<^sub>c cs e\<^sub>2' # s') cs e\<^sub>1')" 
     by (metis iter_refl iter_step)
   with S E show ?case by fastforce
 next
   case (ev\<^sub>k_app2 e\<^sub>2 s e\<^sub>1)
-  then obtain s\<^sub>c c where S: "FApp1\<^sub>k e\<^sub>2 # s = declosure_stack s\<^sub>c \<and> \<Sigma>\<^sub>c = CSC s\<^sub>c c \<and> e\<^sub>1 = declosure c"
+  then obtain s\<^sub>c c where S: "FApp1\<^sub>k e\<^sub>2 # s = declosure_stack s\<^sub>c \<and> \<Sigma>\<^sub>c = SC\<^sub>c s\<^sub>c c \<and> e\<^sub>1 = declosure c"
     by fastforce
-  then obtain cs' e\<^sub>2' s\<^sub>c' where S': "s\<^sub>c = CApp1 cs' e\<^sub>2' # s\<^sub>c' \<and> 
+  then obtain cs' e\<^sub>2' s\<^sub>c' where S': "s\<^sub>c = FApp1\<^sub>c cs' e\<^sub>2' # s\<^sub>c' \<and> 
     e\<^sub>2 = multisubst (map declosure cs') e\<^sub>2' \<and> s = declosure_stack s\<^sub>c'" by fastforce
-  have "CSC (CApp1 cs' e\<^sub>2' # s\<^sub>c') c \<leadsto>\<^sub>c CSE (CApp2 c # s\<^sub>c') cs' e\<^sub>2'" by simp
-  hence "iter (\<leadsto>\<^sub>c) (CSC (CApp1 cs' e\<^sub>2' # s\<^sub>c') c) (CSE (CApp2 c # s\<^sub>c') cs' e\<^sub>2')" 
+  have "SC\<^sub>c (FApp1\<^sub>c cs' e\<^sub>2' # s\<^sub>c') c \<leadsto>\<^sub>c SE\<^sub>c (FApp2\<^sub>c c # s\<^sub>c') cs' e\<^sub>2'" by simp
+  hence "iter (\<leadsto>\<^sub>c) (SC\<^sub>c (FApp1\<^sub>c cs' e\<^sub>2' # s\<^sub>c') c) (SE\<^sub>c (FApp2\<^sub>c c # s\<^sub>c') cs' e\<^sub>2')" 
     by (metis iter_refl iter_step)
   with S S' show ?case by fastforce
 next
   case (ev\<^sub>k_app3 t\<^sub>1 e\<^sub>1 s e\<^sub>2)
-  then obtain s\<^sub>c c\<^sub>2 where S: "FApp2\<^sub>k (Lam\<^sub>d t\<^sub>1 e\<^sub>1) # s = declosure_stack s\<^sub>c \<and> \<Sigma>\<^sub>c = CSC s\<^sub>c c\<^sub>2 \<and> 
+  then obtain s\<^sub>c c\<^sub>2 where S: "FApp2\<^sub>k (Lam\<^sub>d t\<^sub>1 e\<^sub>1) # s = declosure_stack s\<^sub>c \<and> \<Sigma>\<^sub>c = SC\<^sub>c s\<^sub>c c\<^sub>2 \<and> 
     e\<^sub>2 = declosure c\<^sub>2" by fastforce
-  then obtain c s\<^sub>c' where S': "s\<^sub>c = CApp2 c # s\<^sub>c' \<and> Lam\<^sub>d t\<^sub>1 e\<^sub>1 = declosure c \<and> 
+  then obtain c s\<^sub>c' where S': "s\<^sub>c = FApp2\<^sub>c c # s\<^sub>c' \<and> Lam\<^sub>d t\<^sub>1 e\<^sub>1 = declosure c \<and> 
     s = declosure_stack s\<^sub>c'" by fastforce
   from ev\<^sub>k_app3 S S' obtain t' t\<^sub>2 cs where T: "(c :\<^sub>c\<^sub>l Arrow t' t\<^sub>2) \<and> (s\<^sub>c' :\<^sub>c t\<^sub>2 \<rightarrow> t) \<and> 
     latest_environment s\<^sub>c' = Some cs \<and> c\<^sub>2 :\<^sub>c\<^sub>l t'" by fastforce
-  with S' obtain cs' e\<^sub>1' where C: "c = CLam t\<^sub>1 cs' e\<^sub>1' \<and> 
+  with S' obtain cs' e\<^sub>1' where C: "c = Lam\<^sub>c t\<^sub>1 cs' e\<^sub>1' \<and> 
     multisubst (map declosure cs') (Lam\<^sub>d t\<^sub>1 e\<^sub>1') = Lam\<^sub>d t\<^sub>1 e\<^sub>1 \<and> ([t\<^sub>1] \<turnstile>\<^sub>d e\<^sub>1 : t\<^sub>2) \<and> t' = t\<^sub>1 \<and>
     (\<forall>e\<^sub>2. ([] \<turnstile>\<^sub>d e\<^sub>2 : t\<^sub>1) \<longrightarrow> multisubst (map declosure cs') (subst\<^sub>d 0 e\<^sub>2 e\<^sub>1') = subst\<^sub>d 0 e\<^sub>2 e\<^sub>1)" 
       by (metis lam_to_declosure)
   with T S have "subst\<^sub>d 0 e\<^sub>2 e\<^sub>1 = multisubst (map declosure cs') (subst\<^sub>d 0 (declosure c\<^sub>2) e\<^sub>1')" 
     by simp
   with S S' have X: "S\<^sub>k False (FReturn\<^sub>k # s) (subst\<^sub>d 0 e\<^sub>2 e\<^sub>1) = 
-    declosure_state (CSE (CReturn (c\<^sub>2 # cs') # s\<^sub>c') (c\<^sub>2 # cs') e\<^sub>1')" by simp
-  have "CSC (CApp2 (CLam t\<^sub>1 cs' e\<^sub>1') # s\<^sub>c') c\<^sub>2 \<leadsto>\<^sub>c CSE (CReturn (c\<^sub>2 # cs') # s\<^sub>c') (c\<^sub>2 # cs') e\<^sub>1'"
+    destate\<^sub>c (SE\<^sub>c (FReturn\<^sub>c (c\<^sub>2 # cs') # s\<^sub>c') (c\<^sub>2 # cs') e\<^sub>1')" by simp
+  have "SC\<^sub>c (FApp2\<^sub>c (Lam\<^sub>c t\<^sub>1 cs' e\<^sub>1') # s\<^sub>c') c\<^sub>2 \<leadsto>\<^sub>c SE\<^sub>c (FReturn\<^sub>c (c\<^sub>2 # cs') # s\<^sub>c') (c\<^sub>2 # cs') e\<^sub>1'"
     by simp
   with S S' C X show ?case by (metis iter_step iter_refl)
 next
   case (ev\<^sub>k_ret s e)
-  then obtain s\<^sub>c c where S: "FReturn\<^sub>k # s = declosure_stack s\<^sub>c \<and> \<Sigma>\<^sub>c = CSC s\<^sub>c c \<and> e = declosure c" 
+  then obtain s\<^sub>c c where S: "FReturn\<^sub>k # s = declosure_stack s\<^sub>c \<and> \<Sigma>\<^sub>c = SC\<^sub>c s\<^sub>c c \<and> e = declosure c" 
     by fastforce
-  then obtain cs s\<^sub>c' where S': "s\<^sub>c = CReturn cs # s\<^sub>c'" by fastforce
-  have "CSC (CReturn cs # s\<^sub>c') c \<leadsto>\<^sub>c CSC s\<^sub>c' c" by simp
-  hence "iter (\<leadsto>\<^sub>c) (CSC (CReturn cs # s\<^sub>c') c) (CSC s\<^sub>c' c)" by (metis iter_refl iter_step)
+  then obtain cs s\<^sub>c' where S': "s\<^sub>c = FReturn\<^sub>c cs # s\<^sub>c'" by fastforce
+  have "SC\<^sub>c (FReturn\<^sub>c cs # s\<^sub>c') c \<leadsto>\<^sub>c SC\<^sub>c s\<^sub>c' c" by simp
+  hence "iter (\<leadsto>\<^sub>c) (SC\<^sub>c (FReturn\<^sub>c cs # s\<^sub>c') c) (SC\<^sub>c s\<^sub>c' c)" by (metis iter_refl iter_step)
   with S S' show ?case by fastforce
 qed
 
-lemma [simp]: "iter (\<leadsto>\<^sub>k) (declosure_state \<Sigma>\<^sub>c) \<Sigma>\<^sub>s' \<Longrightarrow> \<Sigma>\<^sub>c :\<^sub>c t \<Longrightarrow> 
-  \<exists>\<Sigma>\<^sub>c'. iter (\<leadsto>\<^sub>c) \<Sigma>\<^sub>c \<Sigma>\<^sub>c' \<and> \<Sigma>\<^sub>s' = declosure_state \<Sigma>\<^sub>c'"
-proof (induction "declosure_state \<Sigma>\<^sub>c" \<Sigma>\<^sub>s' arbitrary: \<Sigma>\<^sub>c rule: iter.induct)
+lemma [simp]: "iter (\<leadsto>\<^sub>k) (destate\<^sub>c \<Sigma>\<^sub>c) \<Sigma>\<^sub>s' \<Longrightarrow> \<Sigma>\<^sub>c :\<^sub>c t \<Longrightarrow> 
+  \<exists>\<Sigma>\<^sub>c'. iter (\<leadsto>\<^sub>c) \<Sigma>\<^sub>c \<Sigma>\<^sub>c' \<and> \<Sigma>\<^sub>s' = destate\<^sub>c \<Sigma>\<^sub>c'"
+proof (induction "destate\<^sub>c \<Sigma>\<^sub>c" \<Sigma>\<^sub>s' arbitrary: \<Sigma>\<^sub>c rule: iter.induct)
   case (iter_step \<Sigma>\<^sub>s' \<Sigma>\<^sub>s'')
-  moreover then obtain \<Sigma>\<^sub>c' where X: "iter (\<leadsto>\<^sub>c) \<Sigma>\<^sub>c \<Sigma>\<^sub>c' \<and> \<Sigma>\<^sub>s' = declosure_state \<Sigma>\<^sub>c'" by fastforce
+  moreover then obtain \<Sigma>\<^sub>c' where X: "iter (\<leadsto>\<^sub>c) \<Sigma>\<^sub>c \<Sigma>\<^sub>c' \<and> \<Sigma>\<^sub>s' = destate\<^sub>c \<Sigma>\<^sub>c'" by fastforce
   moreover with iter_step have "\<Sigma>\<^sub>c' :\<^sub>c t" by fastforce
-  ultimately obtain \<Sigma>\<^sub>c'' where "iter (\<leadsto>\<^sub>c) \<Sigma>\<^sub>c' \<Sigma>\<^sub>c'' \<and> \<Sigma>\<^sub>s'' = declosure_state \<Sigma>\<^sub>c''" by fastforce
-  with X have "iter (\<leadsto>\<^sub>c) \<Sigma>\<^sub>c \<Sigma>\<^sub>c'' \<and> \<Sigma>\<^sub>s'' = declosure_state \<Sigma>\<^sub>c''" by (metis iter_append)
+  ultimately obtain \<Sigma>\<^sub>c'' where "iter (\<leadsto>\<^sub>c) \<Sigma>\<^sub>c' \<Sigma>\<^sub>c'' \<and> \<Sigma>\<^sub>s'' = destate\<^sub>c \<Sigma>\<^sub>c''" by fastforce
+  with X have "iter (\<leadsto>\<^sub>c) \<Sigma>\<^sub>c \<Sigma>\<^sub>c'' \<and> \<Sigma>\<^sub>s'' = destate\<^sub>c \<Sigma>\<^sub>c''" by (metis iter_append)
   thus ?case by fastforce
 qed force+
 
-lemma [simp]: "value\<^sub>d (multisubst (map declosure cs) e) \<Longrightarrow> \<exists>c. CSE s cs e \<leadsto>\<^sub>c CSC s c" 
+lemma [simp]: "value\<^sub>d (multisubst (map declosure cs) e) \<Longrightarrow> \<exists>c. SE\<^sub>c s cs e \<leadsto>\<^sub>c SC\<^sub>c s c" 
 proof (induction e)
   case (Var\<^sub>d x)
   then obtain c where "lookup cs x = Some c" by (induction cs x rule: lookup.induct) simp_all
-  hence "CSE s cs (Var\<^sub>d x) \<leadsto>\<^sub>c CSC s c" by simp
+  hence "SE\<^sub>c s cs (Var\<^sub>d x) \<leadsto>\<^sub>c SC\<^sub>c s c" by simp
   thus ?case by fastforce
 next
   case (Const\<^sub>d k)
-  have "CSE s cs (Const\<^sub>d k) \<leadsto>\<^sub>c CSC s (CConst k)" by simp
+  have "SE\<^sub>c s cs (Const\<^sub>d k) \<leadsto>\<^sub>c SC\<^sub>c s (Const\<^sub>c k)" by simp
   thus ?case by fastforce
 next
   case (Lam\<^sub>d t e)
-  have "CSE s cs (Lam\<^sub>d t e) \<leadsto>\<^sub>c CSC s (CLam t cs e)" by simp
+  have "SE\<^sub>c s cs (Lam\<^sub>d t e) \<leadsto>\<^sub>c SC\<^sub>c s (Lam\<^sub>c t cs e)" by simp
   thus ?case by fastforce
 qed simp_all
 
-lemma [simp]: "\<Sigma>\<^sub>c :\<^sub>c t \<Longrightarrow> iter (\<leadsto>\<^sub>k) (declosure_state \<Sigma>\<^sub>c) (S\<^sub>k True [] v) \<Longrightarrow> 
-  \<exists>c. iter (\<leadsto>\<^sub>c) \<Sigma>\<^sub>c (CSC [] c) \<and> declosure c = v"
+lemma [simp]: "\<Sigma>\<^sub>c :\<^sub>c t \<Longrightarrow> iter (\<leadsto>\<^sub>k) (destate\<^sub>c \<Sigma>\<^sub>c) (S\<^sub>k True [] v) \<Longrightarrow> 
+  \<exists>c. iter (\<leadsto>\<^sub>c) \<Sigma>\<^sub>c (SC\<^sub>c [] c) \<and> declosure c = v"
 proof -
-  assume TC: "\<Sigma>\<^sub>c :\<^sub>c t" and "iter (\<leadsto>\<^sub>k) (declosure_state \<Sigma>\<^sub>c) (S\<^sub>k True [] v)"
-  then obtain \<Sigma>\<^sub>c' where E: "iter (\<leadsto>\<^sub>c) \<Sigma>\<^sub>c \<Sigma>\<^sub>c' \<and> S\<^sub>k True [] v = declosure_state \<Sigma>\<^sub>c'" by fastforce
-  then obtain s' c where "[] = declosure_stack s' \<and> \<Sigma>\<^sub>c' = CSC s' c \<and> v = declosure c" by fastforce
+  assume TC: "\<Sigma>\<^sub>c :\<^sub>c t" and "iter (\<leadsto>\<^sub>k) (destate\<^sub>c \<Sigma>\<^sub>c) (S\<^sub>k True [] v)"
+  then obtain \<Sigma>\<^sub>c' where E: "iter (\<leadsto>\<^sub>c) \<Sigma>\<^sub>c \<Sigma>\<^sub>c' \<and> S\<^sub>k True [] v = destate\<^sub>c \<Sigma>\<^sub>c'" by fastforce
+  then obtain s' c where "[] = declosure_stack s' \<and> \<Sigma>\<^sub>c' = SC\<^sub>c s' c \<and> v = declosure c" by fastforce
   moreover hence "s' = []" by simp
-  ultimately have S: "(\<exists>cs e. \<Sigma>\<^sub>c' = CSE [] cs e \<and> v = multisubst (map declosure cs) e) \<or> 
-    (\<exists>c. \<Sigma>\<^sub>c' = CSC [] c \<and> v = declosure c)" by simp
+  ultimately have S: "(\<exists>cs e. \<Sigma>\<^sub>c' = SE\<^sub>c [] cs e \<and> v = multisubst (map declosure cs) e) \<or> 
+    (\<exists>c. \<Sigma>\<^sub>c' = SC\<^sub>c [] c \<and> v = declosure c)" by simp
   with E show ?thesis by fastforce
 qed
 
