06TreeCode/TreeCodeConversion.thy
@@ -8,32 +8,32 @@ primrec encode :: "expr\<^sub>d \<Rightarrow> tree_code list" where
 | "encode (Lam\<^sub>d t e) = [TPushLam (encode e)]"
 | "encode (App\<^sub>d e\<^sub>1 e\<^sub>2) = encode e\<^sub>1 @ encode e\<^sub>2 @ [TApply]"
 
-primrec encode_closure :: "closure \<Rightarrow> tclosure" where
-  "encode_closure (CConst k) = TConst k"
-| "encode_closure (CLam t cs e) = TLam (map encode_closure cs) (encode e)"
+primrec encode_closure :: "closure\<^sub>c \<Rightarrow> tclosure" where
+  "encode_closure (Const\<^sub>c k) = TConst k"
+| "encode_closure (Lam\<^sub>c t cs e) = TLam (map encode_closure cs) (encode e)"
 
-fun vals_from_stack :: "cframe list \<Rightarrow> tclosure list" where
+fun vals_from_stack :: "frame\<^sub>c list \<Rightarrow> tclosure list" where
   "vals_from_stack [] = []"
-| "vals_from_stack (CApp1 cs e # s) = vals_from_stack s"
-| "vals_from_stack (CApp2 c # s) = encode_closure c # vals_from_stack s"
-| "vals_from_stack (CReturn cs # s) = vals_from_stack s"
+| "vals_from_stack (FApp1\<^sub>c cs e # s) = vals_from_stack s"
+| "vals_from_stack (FApp2\<^sub>c c # s) = encode_closure c # vals_from_stack s"
+| "vals_from_stack (FReturn\<^sub>c cs # s) = vals_from_stack s"
 
-fun stack_from_stack :: "cframe list \<Rightarrow> tree_stack_frame list" where
+fun stack_from_stack :: "frame\<^sub>c list \<Rightarrow> tree_stack_frame list" where
   "stack_from_stack [] = []"
-| "stack_from_stack (CApp1 cs e # s) = (case stack_from_stack s of
+| "stack_from_stack (FApp1\<^sub>c cs e # s) = (case stack_from_stack s of
       [] \<Rightarrow> []
     | ((env, cd) # sfs) \<Rightarrow> (env, encode e @ TApply # cd) # sfs)"
-| "stack_from_stack (CApp2 c # s) = (case stack_from_stack s of
+| "stack_from_stack (FApp2\<^sub>c c # s) = (case stack_from_stack s of
       [] \<Rightarrow> []
     | ((env, cd) # sfs) \<Rightarrow> (env, TApply # cd) # sfs)"
-| "stack_from_stack (CReturn cs # s) = (map encode_closure cs, []) # stack_from_stack s"
+| "stack_from_stack (FReturn\<^sub>c cs # s) = (map encode_closure cs, []) # stack_from_stack s"
 
-primrec encode_state :: "closure_state \<Rightarrow> tree_code_state" where
-  "encode_state (CSE s cs e) = 
+primrec encode_state :: "state\<^sub>c \<Rightarrow> tree_code_state" where
+  "encode_state (SE\<^sub>c s cs e) = 
     TS (vals_from_stack s) (case stack_from_stack s of 
         [] \<Rightarrow> []
       | ((env, cd) # sfs) \<Rightarrow> ((env, encode e @ cd) # sfs))"
-| "encode_state (CSC s c) = 
+| "encode_state (SC\<^sub>c s c) = 
     TS (encode_closure c # vals_from_stack s) (stack_from_stack s)"
 
 primrec unzip :: "expr\<^sub>d \<Rightarrow> expr\<^sub>d \<times> expr\<^sub>d list" where
@@ -54,7 +54,7 @@ lemma [simp]: "list_all full_code_closure (encode e)"
 
 lemma [simp]: "full_closure (encode_closure c)"
 proof (induction c)
-  case (CLam t cs e)
+  case (Lam\<^sub>c t cs e)
   thus ?case using list_all_iff by fastforce
 qed simp_all
 
@@ -98,11 +98,11 @@ lemma [simp]: "encode e \<noteq> []"
 lemma [simp]: "unzip e = (e', es) \<Longrightarrow> encode e' @ zip_encode es = encode e"
   by (induction e arbitrary: e' es) (auto split: prod.splits)
 
-lemma [simp]: "vals_from_stack (map (CApp1 cs) (rev es) @ s) = vals_from_stack s"
+lemma [simp]: "vals_from_stack (map (FApp1\<^sub>c cs) (rev es) @ s) = vals_from_stack s"
   by (induction es arbitrary: s) simp_all
 
 lemma [simp]: "stack_from_stack s = (env, cd) # sfs \<Longrightarrow> 
-    stack_from_stack (map (CApp1 cs) (rev es) @ s) = (env, zip_encode es @ cd) # sfs"
+    stack_from_stack (map (FApp1\<^sub>c cs) (rev es) @ s) = (env, zip_encode es @ cd) # sfs"
   by (induction es arbitrary: s cd) simp_all
 
 lemma [dest]: "encode e @ cd' = TLookup x # cd \<Longrightarrow> 
@@ -121,24 +121,24 @@ lemma encode_to_pushlam' [dest]: "encode e @ cd' = TPushLam cd'' # cd \<Longrigh
 lemma [dest]: "encode e @ cd' = TApply # cd \<Longrightarrow> P"
   by (induction e arbitrary: cd') simp_all
 
-lemma [dest]: "encode_closure c = TConst k \<Longrightarrow> c = CConst k"
+lemma [dest]: "encode_closure c = TConst k \<Longrightarrow> c = Const\<^sub>c k"
   by (induction c) simp_all
 
 lemma encode_lam_closure [dest]: "encode_closure c = TLam env cd \<Longrightarrow> (\<And>t cs e. 
-    c = CLam t cs e \<Longrightarrow> env = map encode_closure cs \<Longrightarrow> cd = encode e \<Longrightarrow> P) \<Longrightarrow> P"
+    c = Lam\<^sub>c t cs e \<Longrightarrow> env = map encode_closure cs \<Longrightarrow> cd = encode e \<Longrightarrow> P) \<Longrightarrow> P"
   by (induction c) simp_all
 
-lemma tc_latest_environment [simp]: "s @ CApp1 cs e # s' :\<^sub>c t \<rightarrow> t' \<Longrightarrow> 
+lemma tc_latest_environment [simp]: "s @ FApp1\<^sub>c cs e # s' :\<^sub>c t \<rightarrow> t' \<Longrightarrow> 
   latest_environment s' = Some cs"
 proof (induction s arbitrary: t)
   case (Cons f s)
-  moreover from Cons(2) obtain tt where "s @ CApp1 cs e # s' :\<^sub>c tt \<rightarrow> t'" 
-    by (induction "(f # s) @ CApp1 cs e # s'" t t' rule: typecheck_cstack.induct) simp_all
+  moreover from Cons(2) obtain tt where "s @ FApp1\<^sub>c cs e # s' :\<^sub>c tt \<rightarrow> t'" 
+    by (induction "(f # s) @ FApp1\<^sub>c cs e # s'" t t' rule: typing_stack\<^sub>c.induct) simp_all
   ultimately show ?case by simp
 qed fastforce+
 
 lemma encode_stack_to_lookup [dest]: "stack_from_stack s = (env, TLookup x # cd) # sfs \<Longrightarrow> 
-  \<exists>cs e es s' cd'. s = CApp1 cs e # s' \<and> stack_from_stack s' = (env, cd') # sfs \<and> 
+  \<exists>cs e es s' cd'. s = FApp1\<^sub>c cs e # s' \<and> stack_from_stack s' = (env, cd') # sfs \<and> 
     unzip e = (Var\<^sub>d x, es) \<and> cd = zip_encode es @ TApply # cd'"
 proof (induction s rule: stack_from_stack.induct)
   case (2 cs e s)
@@ -149,7 +149,7 @@ proof (induction s rule: stack_from_stack.induct)
 qed (auto split: list.splits)
 
 lemma encode_stack_to_pushcon [dest]: "stack_from_stack s = (env, TPushCon k # cd) # sfs \<Longrightarrow> 
-  \<exists>cs e es s' cd'. s = CApp1 cs e # s' \<and> stack_from_stack s' = (env, cd') # sfs \<and> 
+  \<exists>cs e es s' cd'. s = FApp1\<^sub>c cs e # s' \<and> stack_from_stack s' = (env, cd') # sfs \<and> 
     unzip e = (Const\<^sub>d k, es) \<and> cd = zip_encode es @ TApply # cd'"
 proof (induction s rule: stack_from_stack.induct)
   case (2 cs e s)
@@ -160,7 +160,7 @@ proof (induction s rule: stack_from_stack.induct)
 qed (auto split: list.splits)
 
 lemma encode_stack_to_pushlam [dest]: "stack_from_stack s = (env, TPushLam cd' # cd) # sfs \<Longrightarrow> 
-  \<exists>cs e es s' t e' cd''. s = CApp1 cs e # s' \<and> stack_from_stack s' = (env, cd'') # sfs \<and> 
+  \<exists>cs e es s' t e' cd''. s = FApp1\<^sub>c cs e # s' \<and> stack_from_stack s' = (env, cd'') # sfs \<and> 
     unzip e = (Lam\<^sub>d t e', es) \<and> cd = zip_encode es @ TApply # cd'' \<and> cd' = encode e'"
 proof (induction s rule: stack_from_stack.induct)
   case (2 cs e s)
@@ -173,49 +173,49 @@ proof (induction s rule: stack_from_stack.induct)
 qed (auto split: list.splits)
 
 lemma encode_stack_to_apply [dest]: "stack_from_stack s = (env, TApply # cd) # sfs \<Longrightarrow> 
-    \<exists>s' c. s = CApp2 c # s' \<and> stack_from_stack s' = (env, cd) # sfs"
+    \<exists>s' c. s = FApp2\<^sub>c c # s' \<and> stack_from_stack s' = (env, cd) # sfs"
   by (induction s rule: stack_from_stack.induct) (auto split: list.splits)
 
 lemma encode_stack_to_return [dest]: "stack_from_stack s = (env, []) # sfs \<Longrightarrow> 
-  (s = [] \<and> env = [] \<and>  sfs = []) \<or> (\<exists>cs s'. s = CReturn cs # s' \<and> env = map encode_closure cs \<and> 
+  (s = [] \<and> env = [] \<and>  sfs = []) \<or> (\<exists>cs s'. s = FReturn\<^sub>c cs # s' \<and> env = map encode_closure cs \<and> 
     sfs = stack_from_stack s')"
   by (induction s rule: stack_from_stack.induct) (auto split: list.splits)
 
 lemma encode_to_lookup [simp]: "encode_state \<Sigma> = TS vs ((env, TLookup x # cd) # sfs) \<Longrightarrow> 
-  (\<exists>s cs e es cd'. \<Sigma> = CSE s cs e \<and> unzip e = (Var\<^sub>d x, es) \<and> 
+  (\<exists>s cs e es cd'. \<Sigma> = SE\<^sub>c s cs e \<and> unzip e = (Var\<^sub>d x, es) \<and> 
     cd = zip_encode es @ cd' \<and> stack_from_stack s = ((env, cd') # sfs) \<and> 
-      vs = vals_from_stack s) \<or> (\<exists>s c cs e es cd'. \<Sigma> = CSC (CApp1 cs e # s) c \<and> 
+      vs = vals_from_stack s) \<or> (\<exists>s c cs e es cd'. \<Sigma> = SC\<^sub>c (FApp1\<^sub>c cs e # s) c \<and> 
         unzip e = (Var\<^sub>d x, es) \<and> cd = zip_encode es @ TApply # cd' \<and> 
           stack_from_stack s = ((env, cd') # sfs) \<and> vs = encode_closure c # vals_from_stack s)"
 proof (induction \<Sigma>)
-  case (CSE s cs e)
+  case (SE\<^sub>c s cs e)
   moreover then obtain cd' where "stack_from_stack s = (env, cd') # sfs \<and> 
     encode e @ cd' = TLookup x # cd" by (auto split: list.splits)
   ultimately show ?case by auto
 qed auto
 
 lemma encode_to_pushcon [simp]: "encode_state \<Sigma> = TS vs ((env, TPushCon k # cd) # sfs) \<Longrightarrow> 
-  (\<exists>s cs e es cd'. \<Sigma> = CSE s cs e \<and> unzip e = (Const\<^sub>d k, es) \<and> 
+  (\<exists>s cs e es cd'. \<Sigma> = SE\<^sub>c s cs e \<and> unzip e = (Const\<^sub>d k, es) \<and> 
     cd = zip_encode es @ cd' \<and> stack_from_stack s = ((env, cd') # sfs) \<and> 
-      vs = vals_from_stack s) \<or> (\<exists>s c cs e es cd'. \<Sigma> = CSC (CApp1 cs e # s) c \<and> 
+      vs = vals_from_stack s) \<or> (\<exists>s c cs e es cd'. \<Sigma> = SC\<^sub>c (FApp1\<^sub>c cs e # s) c \<and> 
         unzip e = (Const\<^sub>d k, es) \<and> cd = zip_encode es @ TApply # cd' \<and> 
           stack_from_stack s = ((env, cd') # sfs) \<and> vs = encode_closure c # vals_from_stack s)"
 proof (induction \<Sigma>)
-  case (CSE s cs e)
+  case (SE\<^sub>c s cs e)
   moreover then obtain cd' where "stack_from_stack s = (env, cd') # sfs \<and> 
     encode e @ cd' = TPushCon k # cd" by (auto split: list.splits)
   ultimately show ?case by auto
 qed auto
 
 lemma encode_to_pushlam [simp]: "encode_state \<Sigma> = TS vs ((env, TPushLam cd' # cd) # sfs) \<Longrightarrow> 
-  (\<exists>s cs e es tt e' cd''. \<Sigma> = CSE s cs e \<and> unzip e = (Lam\<^sub>d tt e', es) \<and> 
+  (\<exists>s cs e es tt e' cd''. \<Sigma> = SE\<^sub>c s cs e \<and> unzip e = (Lam\<^sub>d tt e', es) \<and> 
     cd = zip_encode es @ cd'' \<and> cd' = encode e' \<and> vs = vals_from_stack s \<and> 
       stack_from_stack s = ((env, cd'') # sfs)) \<or> (\<exists>s c cs e es tt e' cd''. 
-        \<Sigma> = CSC (CApp1 cs e # s) c \<and> unzip e = (Lam\<^sub>d tt e', es) \<and> 
+        \<Sigma> = SC\<^sub>c (FApp1\<^sub>c cs e # s) c \<and> unzip e = (Lam\<^sub>d tt e', es) \<and> 
           cd = zip_encode es @ TApply # cd'' \<and> cd' = encode e' \<and> 
             vs = encode_closure c # vals_from_stack s \<and> stack_from_stack s = ((env, cd'') # sfs))"
 proof (induction \<Sigma>)
-  case (CSE s cs e)
+  case (SE\<^sub>c s cs e)
   moreover then obtain cd'' where "stack_from_stack s = (env, cd'') # sfs \<and> 
     encode e @ cd'' = TPushLam cd' # cd" by (auto split: list.splits)
   moreover then obtain es tt e' where "unzip e = (Lam\<^sub>d tt e', es) \<and> cd' = encode e' \<and> 
@@ -224,24 +224,24 @@ proof (induction \<Sigma>)
 qed auto
 
 lemma encode_to_apply [simp]: "encode_state \<Sigma> = TS vs ((env, TApply # cd) # sfs) \<Longrightarrow> 
-  \<exists>s c c'. \<Sigma> = CSC (CApp2 c' # s) c \<and> stack_from_stack s = ((env, cd) # sfs) \<and> 
+  \<exists>s c c'. \<Sigma> = SC\<^sub>c (FApp2\<^sub>c c' # s) c \<and> stack_from_stack s = ((env, cd) # sfs) \<and> 
     vs = encode_closure c # encode_closure c' # vals_from_stack s"
   by (induction \<Sigma>) (auto split: list.splits)
 
 lemma encode_to_return [simp]: "encode_state \<Sigma> = TS vs ((env, []) # sfs) \<Longrightarrow> 
-  (\<exists>c. \<Sigma> = CSC [] c \<and> env = [] \<and> sfs = [] \<and> vs = [encode_closure c]) \<or> 
-    (\<exists>cs s c. \<Sigma> = CSC (CReturn cs # s) c \<and> sfs = stack_from_stack s \<and>
+  (\<exists>c. \<Sigma> = SC\<^sub>c [] c \<and> env = [] \<and> sfs = [] \<and> vs = [encode_closure c]) \<or> 
+    (\<exists>cs s c. \<Sigma> = SC\<^sub>c (FReturn\<^sub>c cs # s) c \<and> sfs = stack_from_stack s \<and>
       env = map encode_closure cs \<and> vs = encode_closure c # vals_from_stack s)"
   by (induction \<Sigma>) (auto split: list.splits)
 
 lemma [simp]: "unzip e = (e', es) \<Longrightarrow> 
-  iter (\<leadsto>\<^sub>c) (CSE s cs e) (CSE (map (CApp1 cs) (rev es) @ s) cs e')"
+  iter (\<leadsto>\<^sub>c) (SE\<^sub>c s cs e) (SE\<^sub>c (map (FApp1\<^sub>c cs) (rev es) @ s) cs e')"
 proof (induction e arbitrary: s es)
   case (App\<^sub>d e1 e2)
   then obtain es' where "unzip e1 = (e', es') \<and> es = e2 # es'" by (auto split: prod.splits)
-  moreover with App\<^sub>d have "iter (\<leadsto>\<^sub>c) (CSE (CApp1 cs e2 # s) cs e1) 
-    (CSE (map (CApp1 cs) (rev (e2 # es')) @ s) cs e')" by simp
-  moreover have "CSE s cs (App\<^sub>d e1 e2) \<leadsto>\<^sub>c CSE (CApp1 cs e2 # s) cs e1" by simp
+  moreover with App\<^sub>d have "iter (\<leadsto>\<^sub>c) (SE\<^sub>c (FApp1\<^sub>c cs e2 # s) cs e1) 
+    (SE\<^sub>c (map (FApp1\<^sub>c cs) (rev (e2 # es')) @ s) cs e')" by simp
+  moreover have "SE\<^sub>c s cs (App\<^sub>d e1 e2) \<leadsto>\<^sub>c SE\<^sub>c (FApp1\<^sub>c cs e2 # s) cs e1" by simp
   ultimately show ?case by (metis iter_step)
 qed simp_all 
 
@@ -254,73 +254,73 @@ theorem correctt [simp]: "encode_state \<Sigma>\<^sub>c \<leadsto>\<^sub>t \<Sig
   \<exists>\<Sigma>\<^sub>c'. iter (\<leadsto>\<^sub>c) \<Sigma>\<^sub>c \<Sigma>\<^sub>c' \<and> \<Sigma>\<^sub>t' = encode_state \<Sigma>\<^sub>c'"
 proof (induction "encode_state \<Sigma>\<^sub>c" \<Sigma>\<^sub>t' rule: evalt.induct)
   case (evt_lookup env x v vs cd sfs)
-  moreover hence "(\<exists>s cs e es cd'. \<Sigma>\<^sub>c = CSE s cs e \<and> unzip e = (Var\<^sub>d x, es) \<and> 
+  moreover hence "(\<exists>s cs e es cd'. \<Sigma>\<^sub>c = SE\<^sub>c s cs e \<and> unzip e = (Var\<^sub>d x, es) \<and> 
     cd = zip_encode es @ cd' \<and> stack_from_stack s = ((env, cd') # sfs) \<and> 
-      vs = vals_from_stack s) \<or> (\<exists>s c cs e es cd'. \<Sigma>\<^sub>c = CSC (CApp1 cs e # s) c \<and> 
+      vs = vals_from_stack s) \<or> (\<exists>s c cs e es cd'. \<Sigma>\<^sub>c = SC\<^sub>c (FApp1\<^sub>c cs e # s) c \<and> 
         unzip e = (Var\<^sub>d x, es) \<and> cd = zip_encode es @ TApply # cd' \<and> 
           stack_from_stack s = ((env, cd') # sfs) \<and> vs = encode_closure c # vals_from_stack s)" 
     using encode_to_lookup by simp
   ultimately show ?case
   proof (induction \<Sigma>\<^sub>c)
-    case (CSE s cs e)
+    case (SE\<^sub>c s cs e)
     then obtain es cd' where E: "unzip e = (Var\<^sub>d x, es) \<and> cd = zip_encode es @ cd' \<and>
       stack_from_stack s = ((env, cd') # sfs) \<and> vs = vals_from_stack s" by auto 
-    hence X: "iter (\<leadsto>\<^sub>c) (CSE s cs e) (CSE (map (CApp1 cs) (rev es) @ s) cs (Var\<^sub>d x))" by simp
-    from CSE obtain t' ts where "(s :\<^sub>c t' \<rightarrow> t) \<and> (cs :\<^sub>c\<^sub>l\<^sub>s ts) \<and>
+    hence X: "iter (\<leadsto>\<^sub>c) (SE\<^sub>c s cs e) (SE\<^sub>c (map (FApp1\<^sub>c cs) (rev es) @ s) cs (Var\<^sub>d x))" by simp
+    from SE\<^sub>c obtain t' ts where "(s :\<^sub>c t' \<rightarrow> t) \<and> (cs :\<^sub>c\<^sub>l\<^sub>s ts) \<and>
       latest_environment s = Some cs \<and> (ts \<turnstile>\<^sub>d e : t')" by fastforce
     with E have "env = map encode_closure cs" by fastforce
-    with CSE obtain c where C: "lookup cs x = Some c \<and> encode_closure c = v" by fastforce
-    with X have "iter (\<leadsto>\<^sub>c) (CSE s cs e) (CSC (map (CApp1 cs) (rev es) @ s) c)" by simp
+    with SE\<^sub>c obtain c where C: "lookup cs x = Some c \<and> encode_closure c = v" by fastforce
+    with X have "iter (\<leadsto>\<^sub>c) (SE\<^sub>c s cs e) (SC\<^sub>c (map (FApp1\<^sub>c cs) (rev es) @ s) c)" by simp
     with E C show ?case by fastforce
   next
-    case (CSC s c)
-    then obtain s' cs e es cd' where S: "s = CApp1 cs e # s' \<and> unzip e = (Var\<^sub>d x, es) \<and>
+    case (SC\<^sub>c s c)
+    then obtain s' cs e es cd' where S: "s = FApp1\<^sub>c cs e # s' \<and> unzip e = (Var\<^sub>d x, es) \<and>
         cd = zip_encode es @ TApply # cd' \<and> stack_from_stack s' = ((env, cd') # sfs) \<and>
           vs = encode_closure c # vals_from_stack s'" by auto
-    hence "iter (\<leadsto>\<^sub>c) (CSE (CApp2 c # s') cs e) 
-      (CSE (map (CApp1 cs) (rev es) @ CApp2 c # s') cs (Var\<^sub>d x))" by simp
-    moreover have "CSC (CApp1 cs e # s') c \<leadsto>\<^sub>c CSE (CApp2 c # s') cs e" by simp
-    ultimately have X: "iter (\<leadsto>\<^sub>c) (CSC (CApp1 cs e # s') c) 
-      (CSE (map (CApp1 cs) (rev es) @ CApp2 c # s') cs (Var\<^sub>d x))" by (metis iter_step)
-    from CSC obtain t' where "(s :\<^sub>c t' \<rightarrow> t) \<and> (c :\<^sub>c\<^sub>l t')" by fastforce
+    hence "iter (\<leadsto>\<^sub>c) (SE\<^sub>c (FApp2\<^sub>c c # s') cs e) 
+      (SE\<^sub>c (map (FApp1\<^sub>c cs) (rev es) @ FApp2\<^sub>c c # s') cs (Var\<^sub>d x))" by simp
+    moreover have "SC\<^sub>c (FApp1\<^sub>c cs e # s') c \<leadsto>\<^sub>c SE\<^sub>c (FApp2\<^sub>c c # s') cs e" by simp
+    ultimately have X: "iter (\<leadsto>\<^sub>c) (SC\<^sub>c (FApp1\<^sub>c cs e # s') c) 
+      (SE\<^sub>c (map (FApp1\<^sub>c cs) (rev es) @ FApp2\<^sub>c c # s') cs (Var\<^sub>d x))" by (metis iter_step)
+    from SC\<^sub>c obtain t' where "(s :\<^sub>c t' \<rightarrow> t) \<and> (c :\<^sub>c\<^sub>l t')" by fastforce
     with S obtain ts t\<^sub>1 t\<^sub>2 where "t' = Arrow t\<^sub>1 t\<^sub>2 \<and> (cs :\<^sub>c\<^sub>l\<^sub>s ts) \<and> (ts \<turnstile>\<^sub>d e : t\<^sub>1) \<and> (s' :\<^sub>c t\<^sub>2 \<rightarrow> t) \<and> 
       latest_environment s' = Some cs" by fastforce
     with S have "env = map encode_closure cs" by fastforce
-    with CSC obtain c' where C: "lookup cs x = Some c' \<and> encode_closure c' = v" by fastforce
-    with X have "iter (\<leadsto>\<^sub>c) (CSC (CApp1 cs e # s') c) 
-      (CSC (map (CApp1 cs) (rev es) @ CApp2 c # s') c')" by simp
+    with SC\<^sub>c obtain c' where C: "lookup cs x = Some c' \<and> encode_closure c' = v" by fastforce
+    with X have "iter (\<leadsto>\<^sub>c) (SC\<^sub>c (FApp1\<^sub>c cs e # s') c) 
+      (SC\<^sub>c (map (FApp1\<^sub>c cs) (rev es) @ FApp2\<^sub>c c # s') c')" by simp
     with S C show ?case by fastforce
   qed
 next
   case (evt_pushcon vs env k cd sfs)
-  hence "(\<exists>s cs e es cd'. \<Sigma>\<^sub>c = CSE s cs e \<and> unzip e = (Const\<^sub>d k, es) \<and> 
+  hence "(\<exists>s cs e es cd'. \<Sigma>\<^sub>c = SE\<^sub>c s cs e \<and> unzip e = (Const\<^sub>d k, es) \<and> 
     cd = zip_encode es @ cd' \<and>stack_from_stack s = ((env, cd') # sfs) \<and> 
-      vs = vals_from_stack s) \<or> (\<exists>s c cs e es cd'. \<Sigma>\<^sub>c = CSC (CApp1 cs e # s) c \<and> 
+      vs = vals_from_stack s) \<or> (\<exists>s c cs e es cd'. \<Sigma>\<^sub>c = SC\<^sub>c (FApp1\<^sub>c cs e # s) c \<and> 
         unzip e = (Const\<^sub>d k, es) \<and> cd = zip_encode es @ TApply # cd' \<and>
           stack_from_stack s = ((env, cd') # sfs) \<and> vs = encode_closure c # vals_from_stack s)" 
     using encode_to_pushcon by simp
   thus ?case
   proof (induction \<Sigma>\<^sub>c)
-    case (CSE s cs e)
+    case (SE\<^sub>c s cs e)
     then obtain es cd' where E: "unzip e = (Const\<^sub>d k, es) \<and> cd = zip_encode es @ cd' \<and> 
       stack_from_stack s = ((env, cd') # sfs) \<and> vs = vals_from_stack s" by auto
-    hence "iter (\<leadsto>\<^sub>c) (CSE s cs e) (CSE (map (CApp1 cs) (rev es) @ s) cs (Const\<^sub>d k))" by simp
-    moreover have "CSE (map (CApp1 cs) (rev es) @ s) cs (Const\<^sub>d k) \<leadsto>\<^sub>c 
-      CSC (map (CApp1 cs) (rev es) @ s) (CConst k)" by simp
-    ultimately have "iter (\<leadsto>\<^sub>c) (CSE s cs e) (CSC (map (CApp1 cs) (rev es) @ s) (CConst k))" by simp
+    hence "iter (\<leadsto>\<^sub>c) (SE\<^sub>c s cs e) (SE\<^sub>c (map (FApp1\<^sub>c cs) (rev es) @ s) cs (Const\<^sub>d k))" by simp
+    moreover have "SE\<^sub>c (map (FApp1\<^sub>c cs) (rev es) @ s) cs (Const\<^sub>d k) \<leadsto>\<^sub>c 
+      SC\<^sub>c (map (FApp1\<^sub>c cs) (rev es) @ s) (Const\<^sub>c k)" by simp
+    ultimately have "iter (\<leadsto>\<^sub>c) (SE\<^sub>c s cs e) (SC\<^sub>c (map (FApp1\<^sub>c cs) (rev es) @ s) (Const\<^sub>c k))" by simp
     with E show ?case by fastforce
   next
-    case (CSC s c)
-    then obtain s' cs e es cd' where S: "s = CApp1 cs e # s' \<and> unzip e = (Const\<^sub>d k, es) \<and> 
+    case (SC\<^sub>c s c)
+    then obtain s' cs e es cd' where S: "s = FApp1\<^sub>c cs e # s' \<and> unzip e = (Const\<^sub>d k, es) \<and> 
         cd = zip_encode es @ TApply # cd' \<and> stack_from_stack s' = ((env, cd') # sfs) \<and>
           vs = encode_closure c # vals_from_stack s'" by auto
-    hence "iter (\<leadsto>\<^sub>c) (CSE (CApp2 c # s') cs e) 
-      (CSE (map (CApp1 cs) (rev es) @ CApp2 c # s') cs (Const\<^sub>d k))" by simp
-    moreover have "CSC (CApp1 cs e # s') c \<leadsto>\<^sub>c CSE (CApp2 c # s') cs e" by simp
-    moreover have "CSE (map (CApp1 cs) (rev es) @ CApp2 c # s') cs (Const\<^sub>d k) \<leadsto>\<^sub>c 
-      CSC (map (CApp1 cs) (rev es) @ CApp2 c # s') (CConst k)" by simp
-    ultimately have "iter (\<leadsto>\<^sub>c) (CSC (CApp1 cs e # s') c)
-      (CSC (map (CApp1 cs) (rev es) @ CApp2 c # s') (CConst k))" 
+    hence "iter (\<leadsto>\<^sub>c) (SE\<^sub>c (FApp2\<^sub>c c # s') cs e) 
+      (SE\<^sub>c (map (FApp1\<^sub>c cs) (rev es) @ FApp2\<^sub>c c # s') cs (Const\<^sub>d k))" by simp
+    moreover have "SC\<^sub>c (FApp1\<^sub>c cs e # s') c \<leadsto>\<^sub>c SE\<^sub>c (FApp2\<^sub>c c # s') cs e" by simp
+    moreover have "SE\<^sub>c (map (FApp1\<^sub>c cs) (rev es) @ FApp2\<^sub>c c # s') cs (Const\<^sub>d k) \<leadsto>\<^sub>c 
+      SC\<^sub>c (map (FApp1\<^sub>c cs) (rev es) @ FApp2\<^sub>c c # s') (Const\<^sub>c k)" by simp
+    ultimately have "iter (\<leadsto>\<^sub>c) (SC\<^sub>c (FApp1\<^sub>c cs e # s') c)
+      (SC\<^sub>c (map (FApp1\<^sub>c cs) (rev es) @ FApp2\<^sub>c c # s') (Const\<^sub>c k))" 
         by (metis iter_step iter_step_after)
     with S show ?case by fastforce
   qed
@@ -328,68 +328,68 @@ next
   case (evt_pushlam vs env cd' cd sfs)
   thus ?case
   proof (induction \<Sigma>\<^sub>c)
-    case (CSE s cs e)
-    hence "encode_state (CSE s cs e) = TS vs ((env, TPushLam cd' # cd) # sfs)" by simp
+    case (SE\<^sub>c s cs e)
+    hence "encode_state (SE\<^sub>c s cs e) = TS vs ((env, TPushLam cd' # cd) # sfs)" by simp
     then obtain es tt e' cd'' where E: "unzip e = (Lam\<^sub>d tt e', es) \<and> 
       cd = zip_encode es @ cd'' \<and> cd' = encode e' \<and> vs = vals_from_stack s \<and> 
         stack_from_stack s = ((env, cd'') # sfs)" 
       using encode_to_pushlam by blast
-    hence "iter (\<leadsto>\<^sub>c) (CSE s cs e) (CSE (map (CApp1 cs) (rev es) @ s) cs (Lam\<^sub>d tt e'))" by simp
-    moreover have "CSE (map (CApp1 cs) (rev es) @ s) cs (Lam\<^sub>d tt e') \<leadsto>\<^sub>c 
-      CSC (map (CApp1 cs) (rev es) @ s) (CLam tt cs e')" by simp
-    ultimately have X: "iter (\<leadsto>\<^sub>c) (CSE s cs e) (CSC (map (CApp1 cs) (rev es) @ s) (CLam tt cs e'))"
+    hence "iter (\<leadsto>\<^sub>c) (SE\<^sub>c s cs e) (SE\<^sub>c (map (FApp1\<^sub>c cs) (rev es) @ s) cs (Lam\<^sub>d tt e'))" by simp
+    moreover have "SE\<^sub>c (map (FApp1\<^sub>c cs) (rev es) @ s) cs (Lam\<^sub>d tt e') \<leadsto>\<^sub>c 
+      SC\<^sub>c (map (FApp1\<^sub>c cs) (rev es) @ s) (Lam\<^sub>c tt cs e')" by simp
+    ultimately have X: "iter (\<leadsto>\<^sub>c) (SE\<^sub>c s cs e) (SC\<^sub>c (map (FApp1\<^sub>c cs) (rev es) @ s) (Lam\<^sub>c tt cs e'))"
       by (metis iter_step_after)
-    from CSE E have "env = map encode_closure cs" by fastforce
-    with CSE E X show ?case by fastforce
+    from SE\<^sub>c E have "env = map encode_closure cs" by fastforce
+    with SE\<^sub>c E X show ?case by fastforce
   next
-    case (CSC s c)
-    hence "encode_state (CSC s c) = TS vs ((env, TPushLam cd' # cd) # sfs)" by simp
-    then obtain s' cs e es tt e' cd'' where S: "s = CApp1 cs e # s' \<and> 
+    case (SC\<^sub>c s c)
+    hence "encode_state (SC\<^sub>c s c) = TS vs ((env, TPushLam cd' # cd) # sfs)" by simp
+    then obtain s' cs e es tt e' cd'' where S: "s = FApp1\<^sub>c cs e # s' \<and> 
       unzip e = (Lam\<^sub>d tt e', es) \<and> cd = zip_encode es @ TApply # cd'' \<and> 
         cd' = encode e' \<and> vs = encode_closure c # vals_from_stack s' \<and> 
           stack_from_stack s' = ((env, cd'') # sfs)" 
       using encode_to_pushlam by fastforce
-    hence "iter (\<leadsto>\<^sub>c) (CSE (CApp2 c # s') cs e) 
-      (CSE (map (CApp1 cs) (rev es) @ CApp2 c # s') cs (Lam\<^sub>d tt e'))" by simp
-    moreover have "CSC (CApp1 cs e # s') c \<leadsto>\<^sub>c CSE (CApp2 c # s') cs e" by simp
-    moreover have "CSE (map (CApp1 cs) (rev es) @ CApp2 c # s') cs (Lam\<^sub>d tt e') \<leadsto>\<^sub>c 
-      CSC (map (CApp1 cs) (rev es) @ CApp2 c # s') (CLam tt cs e')" by simp
-    ultimately have X: "iter (\<leadsto>\<^sub>c) (CSC (CApp1 cs e # s') c) 
-      (CSC (map (CApp1 cs) (rev es) @ CApp2 c # s') (CLam tt cs e'))" 
+    hence "iter (\<leadsto>\<^sub>c) (SE\<^sub>c (FApp2\<^sub>c c # s') cs e) 
+      (SE\<^sub>c (map (FApp1\<^sub>c cs) (rev es) @ FApp2\<^sub>c c # s') cs (Lam\<^sub>d tt e'))" by simp
+    moreover have "SC\<^sub>c (FApp1\<^sub>c cs e # s') c \<leadsto>\<^sub>c SE\<^sub>c (FApp2\<^sub>c c # s') cs e" by simp
+    moreover have "SE\<^sub>c (map (FApp1\<^sub>c cs) (rev es) @ FApp2\<^sub>c c # s') cs (Lam\<^sub>d tt e') \<leadsto>\<^sub>c 
+      SC\<^sub>c (map (FApp1\<^sub>c cs) (rev es) @ FApp2\<^sub>c c # s') (Lam\<^sub>c tt cs e')" by simp
+    ultimately have X: "iter (\<leadsto>\<^sub>c) (SC\<^sub>c (FApp1\<^sub>c cs e # s') c) 
+      (SC\<^sub>c (map (FApp1\<^sub>c cs) (rev es) @ FApp2\<^sub>c c # s') (Lam\<^sub>c tt cs e'))" 
         by (metis iter_step iter_step_after)
-    from CSC S have "env = map encode_closure cs" by fastforce
-    with CSC S X show ?case by fastforce
+    from SC\<^sub>c S have "env = map encode_closure cs" by fastforce
+    with SC\<^sub>c S X show ?case by fastforce
   qed
 next
   case (evt_apply v env' cd' vs env cd sfs)
   hence "encode_state \<Sigma>\<^sub>c = TS (v # TLam env' cd' # vs) ((env, TApply # cd) # sfs)" by simp
-  then obtain s c c' where "\<Sigma>\<^sub>c = CSC (CApp2 c' # s) c \<and> 
+  then obtain s c c' where "\<Sigma>\<^sub>c = SC\<^sub>c (FApp2\<^sub>c c' # s) c \<and> 
     stack_from_stack s = ((env, cd) # sfs) \<and> v = encode_closure c \<and> 
       TLam env' cd' = encode_closure c' \<and> vs = vals_from_stack s" using encode_to_apply by blast
-  moreover then obtain t cs e where "c' = CLam t cs e \<and> env' = map encode_closure cs \<and> 
+  moreover then obtain t cs e where "c' = Lam\<^sub>c t cs e \<and> env' = map encode_closure cs \<and> 
     cd' = encode e" by (metis encode_lam_closure)
-  moreover have "CSC (CApp2 (CLam t cs e) # s) c \<leadsto>\<^sub>c CSE (CReturn (c # cs) # s) (c # cs) e" by simp
-  moreover hence "iter (\<leadsto>\<^sub>c) (CSC (CApp2 (CLam t cs e) # s) c) 
-    (CSE (CReturn (c # cs) # s) (c # cs) e)" by (metis iter_one)
+  moreover have "SC\<^sub>c (FApp2\<^sub>c (Lam\<^sub>c t cs e) # s) c \<leadsto>\<^sub>c SE\<^sub>c (FReturn\<^sub>c (c # cs) # s) (c # cs) e" by simp
+  moreover hence "iter (\<leadsto>\<^sub>c) (SC\<^sub>c (FApp2\<^sub>c (Lam\<^sub>c t cs e) # s) c) 
+    (SE\<^sub>c (FReturn\<^sub>c (c # cs) # s) (c # cs) e)" by (metis iter_one)
   ultimately show ?case using encode_def by fastforce
 next
   case (evt_return vs env sfs)
-  hence R: "(\<exists>c. \<Sigma>\<^sub>c = CSC [] c \<and> env = [] \<and> sfs = [] \<and> vs = [encode_closure c]) \<or> 
-    (\<exists>cs s c. \<Sigma>\<^sub>c = CSC (CReturn cs # s) c \<and> sfs = stack_from_stack s \<and>
+  hence R: "(\<exists>c. \<Sigma>\<^sub>c = SC\<^sub>c [] c \<and> env = [] \<and> sfs = [] \<and> vs = [encode_closure c]) \<or> 
+    (\<exists>cs s c. \<Sigma>\<^sub>c = SC\<^sub>c (FReturn\<^sub>c cs # s) c \<and> sfs = stack_from_stack s \<and>
       env = map encode_closure cs \<and> vs = encode_closure c # vals_from_stack s)" by simp
   thus ?case
-  proof (cases "\<exists>c. \<Sigma>\<^sub>c = CSC [] c \<and> env = [] \<and> sfs = [] \<and> vs = [encode_closure c]")
+  proof (cases "\<exists>c. \<Sigma>\<^sub>c = SC\<^sub>c [] c \<and> env = [] \<and> sfs = [] \<and> vs = [encode_closure c]")
     case True
-    then obtain c where "\<Sigma>\<^sub>c = CSC [] c \<and> env = [] \<and> sfs = [] \<and> vs = [encode_closure c]" 
+    then obtain c where "\<Sigma>\<^sub>c = SC\<^sub>c [] c \<and> env = [] \<and> sfs = [] \<and> vs = [encode_closure c]" 
       by fastforce
-    moreover have "iter (\<leadsto>\<^sub>c) (CSC [] c) (CSC [] c)" by simp
+    moreover have "iter (\<leadsto>\<^sub>c) (SC\<^sub>c [] c) (SC\<^sub>c [] c)" by simp
     ultimately show ?thesis by fastforce
   next
     case False
-    with R obtain cs s c where S: "\<Sigma>\<^sub>c = CSC (CReturn cs # s) c \<and> sfs = stack_from_stack s \<and>
+    with R obtain cs s c where S: "\<Sigma>\<^sub>c = SC\<^sub>c (FReturn\<^sub>c cs # s) c \<and> sfs = stack_from_stack s \<and>
       env = map encode_closure cs \<and> vs = encode_closure c # vals_from_stack s" by fastforce
-    have "CSC (CReturn cs # s) c \<leadsto>\<^sub>c CSC s c" by simp
-    hence "iter (\<leadsto>\<^sub>c) (CSC (CReturn cs # s) c) (CSC s c)" by (metis iter_one)
+    have "SC\<^sub>c (FReturn\<^sub>c cs # s) c \<leadsto>\<^sub>c SC\<^sub>c s c" by simp
+    hence "iter (\<leadsto>\<^sub>c) (SC\<^sub>c (FReturn\<^sub>c cs # s) c) (SC\<^sub>c s c)" by (metis iter_one)
     with S show ?thesis by fastforce
   qed
 qed
@@ -399,20 +399,20 @@ lemma lookup_latest [simp]: "latest_environment s = Some cs \<Longrightarrow>
   by (induction s rule: stack_from_stack.induct) (auto split: list.splits)
 
 theorem completet [simp]: "\<Sigma> \<leadsto>\<^sub>c \<Sigma>' \<Longrightarrow> \<Sigma> :\<^sub>c t \<Longrightarrow> iter (\<leadsto>\<^sub>t) (encode_state \<Sigma>) (encode_state \<Sigma>')"
-proof (induction \<Sigma> \<Sigma>' rule: evalc.induct)
-  case (evc_var cs x c s)
+proof (induction \<Sigma> \<Sigma>' rule: eval\<^sub>c.induct)
+  case (ev\<^sub>c_var cs x c s)
   then obtain t' ts where "(s :\<^sub>c t' \<rightarrow> t) \<and> (cs :\<^sub>c\<^sub>l\<^sub>s ts) \<and> latest_environment s = Some cs \<and> 
     lookup ts x = Some t'" by fastforce
   then obtain cd sfs where S: "stack_from_stack s = (map encode_closure cs, cd) # sfs" 
     by (metis lookup_latest)
-  with evc_var have "TS (vals_from_stack s) ((map encode_closure cs, TLookup x # cd) # sfs) \<leadsto>\<^sub>t 
+  with ev\<^sub>c_var have "TS (vals_from_stack s) ((map encode_closure cs, TLookup x # cd) # sfs) \<leadsto>\<^sub>t 
     TS (encode_closure c # vals_from_stack s) ((map encode_closure cs, cd) # sfs)" by simp
   hence "iter (\<leadsto>\<^sub>t) (TS (vals_from_stack s) ((map encode_closure cs, TLookup x # cd) # sfs))
     (TS (encode_closure c # vals_from_stack s) ((map encode_closure cs, cd) # sfs))" 
       by (metis iter_one)
     with S show ?case by simp
 next
-  case (evc_con s cs k)
+  case (ev\<^sub>c_con s cs k)
   then obtain ts where "(s :\<^sub>c Num \<rightarrow> t) \<and> (cs :\<^sub>c\<^sub>l\<^sub>s ts) \<and> latest_environment s = Some cs" 
     by fastforce
   then obtain cd sfs where S: "stack_from_stack s = (map encode_closure cs, cd) # sfs" 
@@ -423,7 +423,7 @@ next
     (TS (TConst k # vals_from_stack s) ((map encode_closure cs, cd) # sfs))" by (metis iter_one)
   with S show ?case by simp
 next
-  case (evc_lam s cs tt e)
+  case (ev\<^sub>c_lam s cs tt e)
   then obtain t' ts where "(s :\<^sub>c t' \<rightarrow> t) \<and> (cs :\<^sub>c\<^sub>l\<^sub>s ts) \<and> latest_environment s = Some cs \<and>
     (ts \<turnstile>\<^sub>d Lam\<^sub>d tt e : t')" by fastforce
   then obtain cd sfs where S: "stack_from_stack s = (map encode_closure cs, cd) # sfs" 
@@ -437,21 +437,21 @@ next
         ((map encode_closure cs, cd) # sfs))" by (metis iter_one)
   with S show ?case by (simp add: encode_def)
 next
-  case (evc_app s cs e\<^sub>1 e\<^sub>2)
+  case (ev\<^sub>c_app s cs e\<^sub>1 e\<^sub>2)
   then obtain t' ts where "(s :\<^sub>c t' \<rightarrow> t) \<and> (cs :\<^sub>c\<^sub>l\<^sub>s ts) \<and> latest_environment s = Some cs \<and>
     (ts \<turnstile>\<^sub>d App\<^sub>d e\<^sub>1 e\<^sub>2 : t')" by fastforce
   then obtain cd sfs where S: "stack_from_stack s = (map encode_closure cs, cd) # sfs" 
     by (metis lookup_latest)
   then show ?case by simp
 next
-  case (retc_app1 cs e\<^sub>2 s c\<^sub>1)
+  case (ret\<^sub>c_app1 cs e\<^sub>2 s c\<^sub>1)
   then obtain ts t\<^sub>1 t\<^sub>2 where "(cs :\<^sub>c\<^sub>l\<^sub>s ts) \<and> (ts \<turnstile>\<^sub>d e\<^sub>2 : t\<^sub>1) \<and> (s :\<^sub>c t\<^sub>2 \<rightarrow> t) \<and>
     latest_environment s = Some cs \<and> (c\<^sub>1 :\<^sub>c\<^sub>l Arrow t\<^sub>1 t\<^sub>2)" by blast
   then obtain cd sfs where "stack_from_stack s = (map encode_closure cs, cd) # sfs" 
     by (metis lookup_latest)
   thus ?case by simp
 next
-  case (retc_app2 t\<^sub>1 cs e\<^sub>1 s c\<^sub>2)
+  case (ret\<^sub>c_app2 t\<^sub>1 cs e\<^sub>1 s c\<^sub>2)
   then obtain ts t\<^sub>2 cs' where "(cs :\<^sub>c\<^sub>l\<^sub>s ts) \<and> (insert_at 0 t\<^sub>1 ts \<turnstile>\<^sub>d e\<^sub>1 : t\<^sub>2) \<and> (s :\<^sub>c t\<^sub>2 \<rightarrow> t) \<and> 
     latest_environment s = Some cs' \<and> (c\<^sub>2 :\<^sub>c\<^sub>l t\<^sub>1)" by blast
   then obtain cd sfs where S: "stack_from_stack s = (map encode_closure cs', cd) # sfs" 
@@ -468,7 +468,7 @@ next
     by (metis iter_one)
   with S show ?case by (simp add: encode_def)
 next
-  case (retc_ret cs s c)
+  case (ret\<^sub>c_ret cs s c)
   have "TS (encode_closure c # vals_from_stack s) 
     ((map encode_closure cs, []) # stack_from_stack s) \<leadsto>\<^sub>t
       TS (encode_closure c # vals_from_stack s) (stack_from_stack s)" by simp
